core/effect_interpolation_try2.v
@@ -1,0 +1,2163 @@
+Require Import Events. (*is needed for some definitions (loc_unmapped etc*)
+Require Import Memory.
+Require Import Coqlib.
+Require Import Integers.
+Require Import Values.
+Require Import Maps.
+Require Import Axioms.
+
+
+Require Import reach.
+Require Import effect_simulations.
+Require Import effect_simulations_lemmas.
+Require Import mem_lemmas.
+Require Import mem_interpolation_defs.
+Require Import mem_interpolation_II.
+Load mem_interpolation_II3.
+Require Import FiniteMaps.
+Require Import StructuredInjections.
+
+Require Import pure.
+Require Import full_composition.
+
+
+(****************************
+ *         Tactics          *
+ ****************************)
+Lemma locT_localmap: forall mu b2 b d,
+                       SM_wd mu ->
+                       local_of mu b = Some (b2, d) ->
+                       locBlocksTgt mu b2 = true.
+  intros.
+  eapply H in H0. destruct H0 as [locS locT]; auto.
+Qed.
+Lemma locS_localmap: forall mu b p,
+                       SM_wd mu ->
+                       local_of mu b = Some p ->
+                       locBlocksSrc mu b = true.
+  intros. destruct p.
+  eapply H in H0. destruct H0 as [locS locT]; auto.
+Qed.
+Lemma locS_externmap: forall mu b p,
+                        SM_wd mu ->
+                        extern_of mu b = Some p ->
+                        locBlocksSrc mu b = false.
+  intros. destruct (locBlocksSrc mu b) eqn:locS; trivial.
+  destruct p; eapply H in H0. destruct H0 as [extS extT].
+  destruct H as [H ?].
+  destruct (H b); 
+    [rewrite locS in H0 | rewrite extS in H0]; discriminate.
+Qed.
+Lemma locT_externmap: forall mu b b2 d,
+                        SM_wd mu ->
+                        extern_of mu b = Some (b2, d) ->
+                        locBlocksTgt mu b2 = false.
+  intros. destruct (locBlocksTgt mu b2) eqn:locT; trivial.
+  eapply H in H0. destruct H0 as [extS extT].
+  destruct H as [HS HT ?].
+  destruct (HT b2) as [H | H];
+    [rewrite locT in H | rewrite extT in H]; discriminate.
+Qed.
+Lemma validT_externmap: forall mu b2 b1 d m1 m2,
+                          SM_wd mu ->
+                          sm_valid mu m1 m2 ->
+                          extern_of mu b1 = Some (b2,d) ->
+                          Mem.valid_block m2 b2.
+  intros. apply H0.  unfold RNG, DomTgt. eapply H in H1. 
+  destruct H1. rewrite H2; apply orb_true_r.
+Qed.
+
+Lemma validT_localmap: forall mu b2 b1 d m1 m2,
+                          SM_wd mu ->
+                          sm_valid mu m1 m2 ->
+                          local_of mu b1 = Some (b2,d) ->
+                          Mem.valid_block m2 b2.
+  intros. apply H0.  unfold RNG, DomTgt. eapply H in H1. 
+  destruct H1. rewrite H2; apply orb_true_l.
+Qed.
+Lemma validS_externmap: forall mu b1 p m1 m2,
+                          SM_wd mu ->
+                          sm_valid mu m1 m2 ->
+                          extern_of mu b1 = Some p ->
+                          Mem.valid_block m1 b1.
+  intros. apply H0.  unfold DOM, DomSrc. destruct p; eapply H in H1. 
+  destruct H1. rewrite H1; apply orb_true_r.
+Qed.
+
+Lemma validS_localmap: forall mu b1 p m1 m2,
+                          SM_wd mu ->
+                          sm_valid mu m1 m2 ->
+                          local_of mu b1 = Some p ->
+                          Mem.valid_block m1 b1.
+  intros. apply H0.  unfold DOM, DomSrc. destruct p; eapply H in H1. 
+  destruct H1. rewrite H1; apply orb_true_l.
+Qed.
+Lemma loc_ext_map: forall mu b1 b1' b2 d d',
+                     SM_wd mu ->
+                     local_of mu b1 = Some (b2, d) ->
+                     extern_of mu b1' = Some (b2, d') ->
+                     False.
+  intros. apply H in H0; apply H in H1; destruct H0, H1.
+  destruct H as [HS HT ?]; destruct (HT b2).
+  rewrite H2 in H; inversion H.
+  rewrite H3 in H; inversion H.
+Qed.
+
+
+Ltac auto_sm:= 
+               match goal with
+                   | _ => solve [eapply locS_localmap; eassumption]
+                   | _ => solve [eapply locT_localmap; eassumption]
+                   | _ => solve [eapply locS_externmap; eassumption]
+                   | _ => solve [eapply locT_externmap; eassumption]
+                   | [ H: local_of ?mu _ = Some (?b2, _ )|- Mem.valid_block _ ?b2 ] => 
+                     solve[eapply (validT_localmap mu b2); eassumption]
+                   | [ H: local_of ?mu ?b1 = Some _ |- Mem.valid_block _ ?b1 ] => 
+                     solve[eapply (validS_localmap mu b1); eassumption]
+                   | [ H: extern_of ?mu _ = Some (?b2, _ )|- Mem.valid_block _ ?b2 ] => 
+                     solve[eapply (validT_externmap mu b2); eassumption]
+                   | [ H: extern_of ?mu ?b1 = Some _ |- Mem.valid_block _ ?b1 ] => 
+                     solve[eapply (validS_externmap mu b1); eassumption]
+                   | [|- as_inj ?mu ?b1 = _ ] => solve[apply (local_in_all mu); assumption]
+                   | [loc: local_of ?mu _ = Some (?b2 , _),
+                      ext: extern_of ?mu _ = Some (?b2 , _)|- False ] => 
+                     solve[ eapply (loc_ext_map mu); eassumption]
+               end.
+
+
+
+Lemma EFF_interp_II_strong: 
+  forall m1 m2 nu12 
+         (MInj12 : Mem.inject (as_inj nu12) m1 m2) m1'
+         (Fwd1: mem_forward m1 m1') nu23 m3
+         (MInj23 : Mem.inject (as_inj nu23) m2 m3) m3'
+         (Fwd3: mem_forward m3 m3')
+         nu' (WDnu' : SM_wd nu')
+         (SMvalNu' : sm_valid nu' m1' m3')
+         (MemInjNu' : Mem.inject (as_inj nu') m1' m3')
+         (ExtIncr: extern_incr (compose_sm nu12 nu23) nu')
+         (Pure: pure_comp_ext nu12 nu23 m1 m2)
+         (SMV12: sm_valid nu12 m1 m2)
+         (SMV23: sm_valid nu23 m2 m3)
+         (UnchPrivSrc: Mem.unchanged_on 
+                         (fun b ofs => locBlocksSrc (compose_sm nu12 nu23) b = true /\ 
+                                       pubBlocksSrc (compose_sm nu12 nu23) b = false) m1 m1') 
+         (UnchLOOR13: Mem.unchanged_on (local_out_of_reach (compose_sm nu12 nu23) m1) m3 m3')
+         (GlueInvNu: SM_wd nu12 /\ SM_wd nu23 /\
+                     locBlocksTgt nu12 = locBlocksSrc nu23 /\
+                     extBlocksTgt nu12 = extBlocksSrc nu23 /\
+                     (forall b, pubBlocksTgt nu12 b = true -> 
+                                pubBlocksSrc nu23 b = true) /\
+                     (forall b, frgnBlocksTgt nu12 b = true -> 
+                                frgnBlocksSrc nu23 b = true))
+         (Norm12: forall b1 b2 d1, extern_of nu12 b1 = Some(b2,d1) ->
+                                   exists b3 d2, extern_of nu23 b2 = Some(b3, d2))
+         (full: full_ext nu12 nu23),
+  exists m2', exists nu12', exists nu23', nu'=compose_sm nu12' nu23' /\
+                                          extern_incr nu12 nu12' /\ extern_incr nu23 nu23' /\
+                                          pure_comp_ext nu12' nu23' m1' m2' /\
+                                          Mem.inject (as_inj nu12') m1' m2' /\ mem_forward m2 m2' /\
+                                          Mem.inject (as_inj nu23') m2' m3' /\
+                                          sm_valid nu12' m1' m2' /\ sm_valid nu23' m2' m3' /\
+                                          (SM_wd nu12' /\ SM_wd nu23' /\
+                                           locBlocksTgt nu12' = locBlocksSrc nu23' /\
+                                           extBlocksTgt nu12' = extBlocksSrc nu23' /\
+                                           (forall b, pubBlocksTgt nu12' b = true -> 
+                                                      pubBlocksSrc nu23' b = true) /\
+                                           (forall b, frgnBlocksTgt nu12' b = true -> 
+                                                      frgnBlocksSrc nu23' b = true)) /\
+                                          (forall b1 b2 d1, extern_of nu12' b1 = Some(b2,d1) ->
+                                                            exists b3 d2, extern_of nu23' b2 = Some(b3, d2)) /\ 
+                                          Mem.unchanged_on (fun b ofs => locBlocksSrc nu23 b = true /\ 
+                                                                         pubBlocksSrc nu23 b = false) m2 m2' /\
+                                          Mem.unchanged_on (local_out_of_reach nu12 m1) m2 m2' /\
+                                          (*             Mem.unchanged_on (local_out_of_reach nu23 m2) m3 m3' /\*)
+                                          (forall b1 b2 d1, as_inj nu12' b1 = Some(b2,d1) -> 
+                                                            as_inj nu12 b1 = Some(b2,d1) \/
+                                                            exists b3 d, as_inj nu' b1 = Some(b3,d)) /\
+                                          (forall b2 b3 d2, as_inj nu23' b2 = Some(b3,d2) -> 
+                                                            as_inj nu23 b2 = Some(b3,d2) \/
+                                                            exists b1 d, as_inj nu' b1 = Some(b3,d)).
+(*                   (forall b1 b2 ofs2, as_inj nu12' b1 = Some(b2,ofs2) -> 
+                     (as_inj nu12 b1 = Some (b2,ofs2)) \/
+                     (b1 = Mem.nextblock m1 /\ b2 = Mem.nextblock m2 /\ ofs2 = 0) \/ 
+                     (exists m, (b1 = Mem.nextblock m1 + m /\ b2=Mem.nextblock m2 + m)%positive /\ ofs2=0)) /\
+                   (forall b2 b3 ofs3, as_inj nu23' b2 = Some(b3,ofs3) -> 
+                     (as_inj nu23 b2 = Some (b3,ofs3)) \/
+                     (b2 = Mem.nextblock m2 /\ as_inj nu' (Mem.nextblock m1) = Some(b3,ofs3)) \/
+                     (exists m, (b2 = Mem.nextblock m2 + m)%positive /\ 
+                            as_inj nu' ((Mem.nextblock m1+m)%positive) = Some(b3,ofs3))). *)
+Proof. intros.
+       (****************************
+        * Preparing the hypothesis *
+        ****************************)
+       destruct GlueInvNu as [SMWD12 [SMWD23 GlueInv]].
+
+       (***************************************
+        * Construct the injections and memory *
+        ***************************************)
+       remember (extern_of nu12) as j;
+         remember (extern_of nu23) as k;
+         remember (extern_of nu') as l';
+         remember (Mem.nextblock m2) as sizeM2;
+         remember (extBlocksSrc nu') as extS12;
+         remember (bconcat (extBlocksTgt nu12) (extBlocksSrc nu') sizeM2) as extT12;
+         remember (bconcat (extBlocksSrc nu23) (extBlocksSrc nu') sizeM2) as extS23;
+         remember (extBlocksTgt nu') as extT23;
+         remember (mkInjections (Mem.nextblock m2) j k l') as output;
+         destruct output as [j' k'].
+       remember (change_ext nu12 extS12 extT12 j') as nu12';
+         remember (change_ext nu23 extS23 extT23 k') as nu23'.
+       remember (as_inj nu12') as j12'.
+       remember (mem_add nu12 nu23 j12' m1 m1' m2) as m2';
+       exists m2', nu12', nu23'.
+       
+       (************************************************
+        * Proving some properties of my construction   *
+        ************************************************)
+       
+       (* compose_sm *)
+       assert (compose: nu' = compose_sm nu12' nu23').
+       { rewrite Heqnu12', Heqnu23'. (*clear - ExtIncr full. *)
+         destruct ExtIncr as [extincr [? [? [? [? [? [? [? [? ? ]]]]]]]]].
+         unfold compose_sm, change_ext; destruct nu12, nu23, nu'; simpl in *; f_equal; auto.
+         eapply (MKIcomposition j k (extern_of1)); subst; eauto.
+         intros b p H.  destruct p.
+         eapply SMV23. eapply as_inj_DomRng.
+         unfold as_inj, join; simpl; rewrite H; eauto.
+         apply SMWD23. 
+       }
+       
+       (* extern_incr nu12 nu12' *)
+       assert (ExtIncr12: extern_incr nu12 nu12').
+       { unfold extern_incr; simpl.
+         subst nu12' j k extS12 extT12; destruct nu12;
+         unfold extern_incr; simpl.
+         destruct ExtIncr as [extincr [? [extS [extT [? [? [? [? [? ? ]]]]]]]]].
+         simpl in *.
+         intuition.
+         eapply MKI_incr12; eauto.
+         apply bconcat_larger1; exact H9.
+       }
+
+       (* extern_incr nu23 nu23' *)
+       assert (ExtIncr23: extern_incr nu23 nu23').
+       { unfold extern_incr; simpl.
+         subst nu23' j k extS23 extT23; destruct nu23;
+         unfold extern_incr; simpl.
+         destruct ExtIncr as [extincr [? [extS [extT [? [? [? [? [? ? ]]]]]]]]].
+         simpl in *.
+         intuition.
+         eapply MKI_incr23; eauto.
+         apply bconcat_larger1; auto.
+       }
+
+       (* mem_forward m2 m2' *)
+       assert (Fwd2: mem_forward m2 m2').
+       { subst m2'. unfold mem_forward; split.
+         + unfold Mem.valid_block in *.
+           rewrite mem_add_nbx.
+           unfold mem_add_nb.
+           xomega.
+         + intros ofs per. 
+           unfold Mem.perm. rewrite (mem_add_accx nu12 nu23 j12' m1 m1' m2); unfold mem_add_acc.
+           destruct (valid_dec m2 b); try contradiction.
+           destruct (locBlocksSrc nu23 b) eqn: loc23.
+           destruct (pubBlocksSrc nu23 b) eqn: pub23; trivial.
+           destruct (source (local_of nu12) m1 b ofs) eqn:sour; trivial; destruct p.
+           destruct (pubBlocksSrc nu12 b0) eqn: pub12; trivial.
+           symmetry in sour. apply source_SomeE in sour.
+           destruct sour as [b1 [delta' [ofs1 [invertible [leq [mapj [mperm ofs_add]]]]]]].
+           subst ofs; intros H0. eapply MInj12.
+           apply local_in_all; eauto.
+           eapply Fwd1; auto.
+           inversion invertible; subst z b0; auto.
+           
+           destruct (source (as_inj nu12) m1 b ofs) eqn:sour;
+             try solve[destruct (as_inj nu23 b); intros HH;try destruct p; trivial; inversion HH].
+           destruct p.
+           intros H0.
+           symmetry in sour. apply source_SomeE in sour.
+           destruct sour as [b1 [delta' [ofs1 [invertible [leq [mapj [mperm ofs_add]]]]]]].
+           subst ofs; eapply MInj12; eauto.
+           eapply Fwd1; auto.
+           inversion invertible; subst z b0; auto.
+       }
+
+       (* Mem.unchanged_on private m2 *)
+       assert (UnchPrivSrc12 : Mem.unchanged_on
+                   (fun (b : block) (_ : Z) =>
+                      locBlocksSrc nu23 b = true /\ pubBlocksSrc nu23 b = false) m2 m2').
+       { subst m2'. constructor. 
+         + intros b ofs k0 p [locS pubS] bval; unfold Mem.perm.
+           rewrite (mem_add_accx nu12 nu23 j12' m1 m1' m2); unfold mem_add_acc.
+           rewrite locS, pubS.
+           destruct (valid_dec m2 b); try solve[contradict bval;trivial].
+           split; auto.
+         + intros b ofs [locS pubS] mperm.
+           rewrite (mem_add_contx nu12 nu23 j12' m1 m1' m2); unfold mem_add_cont.
+           rewrite locS, pubS.
+           destruct (valid_dec m2 b); try solve[trivial].
+           (*Invalid case*) apply Mem.perm_valid_block in mperm; contradiction.
+       }
+       
+       (*Mem.unchanged_on local_out_of_reach 12*)
+       assert (UnchLOOR12: Mem.unchanged_on (local_out_of_reach nu12 m1) m2 m2').
+       { subst m2'.
+         unfold local_out_of_reach.
+         constructor. 
+         + intros b ofs k0 p [locT mapcondition] bval; unfold Mem.perm.
+           rewrite (mem_add_accx nu12 nu23 j12' m1 m1' m2); 
+                 unfold mem_add_acc.
+           destruct (valid_dec m2 b); try solve[contradict bval;trivial].
+           assert (locS: locBlocksSrc nu23 b = true ) by
+               (destruct GlueInv as [glue1 rest]; rewrite glue1 in locT; trivial).
+           rewrite locS.
+           destruct (pubBlocksSrc nu23 b) eqn:pubS;
+             destruct (source (local_of nu12) m1 b ofs) eqn:sour;
+             try solve [split;auto].
+           - symmetry in sour. apply source_SomeE in sour;
+             destruct sour as [b0 [d0 [ofs0 [invert [bval' [map12 [mparm of_eq] ]]]]]].
+             subst p0 ofs.
+             apply mapcondition in map12. clear mapcondition.
+             destruct map12 as [mperm1 | pubS1].
+             * contradict mperm1. replace (ofs0 + d0 - d0) with ofs0 by omega; trivial.
+             * rewrite pubS1; split; auto.
+         + intros b ofs [locT mapcondition] mperm; unfold Mem.perm.
+           rewrite (mem_add_contx nu12 nu23 j12' m1 m1' m2); 
+                 unfold mem_add_cont.
+           destruct (valid_dec m2 b).
+           - assert (locS: locBlocksSrc nu23 b = true ) by
+                 (destruct GlueInv as [glue1 rest]; rewrite glue1 in locT; trivial).
+             rewrite locS.
+             destruct (pubBlocksSrc nu23 b) eqn:pubS;
+               destruct (source (local_of nu12) m1 b ofs) eqn:sour;
+               try solve [split;auto].
+             symmetry in sour. apply source_SomeE in sour;
+              destruct sour as [b0 [d0 [ofs0 [invert [bval' [map12 [mparm of_eq] ]]]]]].
+             subst p ofs.
+             apply mapcondition in map12. clear mapcondition.
+             destruct map12 as [mperm1 | pubS1].
+             * contradict mperm1. replace (ofs0 + d0 - d0) with ofs0 by omega; trivial.
+             * rewrite pubS1; split; auto.
+           - (*Invalid case*) apply Mem.perm_valid_block in mperm; contradiction.
+       }
+       (*Mem.unchanged_on local_out_of_reach 23*)
+       assert (UnchLOOR23: Mem.unchanged_on (local_out_of_reach nu23 m2) m3 m3').
+       { unfold local_out_of_reach; split; intros.
+         + move UnchLOOR13 at bottom; unfold local_out_of_reach in UnchLOOR13.
+           apply UnchLOOR13; auto.
+           destruct H; split.
+           - unfold compose_sm; trivial.
+           - unfold compose_sm; simpl; intros.
+             unfold compose_meminj in H2. 
+             destruct (local_of nu12 b0) eqn:maploc12; try solve[inversion H2].
+             destruct p0. destruct (local_of nu23 b1) eqn:maploc23; try solve[inversion H2].
+             destruct p0. inversion H2; subst b2 delta; clear H2.
+             eapply H1 in maploc23.
+             destruct maploc23.
+             * left. intros mperm.
+               apply H2. replace (ofs - z0) with ((ofs - (z + z0)) + z) by xomega. 
+               eapply MInj12; eauto. 
+               apply local_in_all; eauto. 
+             * right. destruct (pubBlocksSrc nu12 b0) eqn:pubS12; trivial.
+               apply SMWD12 in pubS12. destruct pubS12 as [b2 [ofs' [maploc12' pubT12]]].
+               rewrite maploc12 in maploc12'; inversion maploc12'; subst b1 z.
+               apply GlueInv in pubT12. rewrite pubT12 in H2; inversion H2.
+         + move UnchLOOR13 at bottom; unfold local_out_of_reach in UnchLOOR13.
+           apply UnchLOOR13; auto.
+           destruct H; split.
+           - unfold compose_sm; trivial.
+           - unfold compose_sm; simpl; intros.
+             unfold compose_meminj in H2. 
+             destruct (local_of nu12 b0) eqn:maploc12; try solve[inversion H2].
+             destruct p. destruct (local_of nu23 b1) eqn:maploc23; try solve[inversion H2].
+             destruct p. inversion H2; subst b2 delta; clear H2.
+             eapply H1 in maploc23.
+             destruct maploc23.
+             * left. intros mperm.
+               apply H2. replace (ofs - z0) with ((ofs - (z + z0)) + z) by xomega. 
+               eapply MInj12; eauto. 
+               apply local_in_all; eauto. 
+             * right. destruct (pubBlocksSrc nu12 b0) eqn:pubS12; trivial.
+               apply SMWD12 in pubS12. destruct pubS12 as [b2 [ofs' [maploc12' pubT12]]].
+               rewrite maploc12 in maploc12'; inversion maploc12'; subst b1 z.
+               apply GlueInv in pubT12. rewrite pubT12 in H2; inversion H2.
+       }
+       
+       (* pure_comp_ext nu12' nu23' m1' m2 *)
+       assert (Pure': pure_comp_ext nu12' nu23' m1' m2').
+       { unfold pure_comp_ext.
+         subst nu12' nu23' m2'. rewrite ext_change_ext, ext_change_ext.
+         split.
+         + unfold pure_composition_locat.
+           clear - Heqoutput Pure Heqj Heqj12' Heqk SMV12 SMV23 SMWD23 SMWD12 MemInjNu'.
+           inversion Heqoutput. intros. 
+           unfold add_inj in H.
+           destruct (k b2) eqn:kmap.
+           - destruct p. inversion H. subst b z. 
+             rewrite Heqk in kmap. 
+             unfold valid_location in H2.
+             unfold Mem.perm in H2. rewrite mem_add_accx in H2.
+             unfold mem_add_acc in H2. 
+             assert (notloc: locBlocksSrc nu23 b2 = false) by auto_sm.
+             rewrite notloc in H2.
+             destruct (valid_dec m2 b2).
+             destruct (source (as_inj nu12) m1 b2 delta) eqn:sour.
+             * symmetry in sour; apply source_SomeE in sour.
+               destruct sour as [b1 [delta0 [ofs1 [pair [bval1 [jmap12' [mperm' d_eq]]]]]]].
+               exists b1, delta0.
+               subst p j12'.
+               
+               assert (jmap: j b1 = Some (b2, delta0))by admit. (* because k maps b2 and jmap12'*)
+               unfold add_inj. rewrite jmap; split; auto.
+               unfold valid_location. 
+               subst delta. replace (ofs1 + delta0 - delta0) with ofs1 by omega. auto.
+             * unfold as_inj, join in H2; rewrite kmap in H2. 
+               inversion H2.
+             * contradict n. apply SMV23. unfold DOM, DomSrc. apply SMWD23 in kmap.
+               destruct kmap as [extS extT]; rewrite extS; apply orb_true_r.
+           - idtac.
+             Lemma shiftS_Some: forall j sh b1 p,
+                                  (j << sh) b1 = Some p ->
+                                  (b1 > sh)%positive /\ j (b1 - sh)%positive = Some p.
+               unfold shiftS. intros.
+               destruct (b1 ?= sh)%positive eqn:ineq; inversion H.
+               split; trivial.
+             Qed.
+             apply shiftS_Some in H; destruct H as [ineq lmap'].
+             apply pure_filter_Some in lmap'; destruct lmap' as [jNone lmap'].
+              generalize H2; unfold valid_location; intros.
+             unfold Mem.perm in H3.
+             rewrite mem_add_accx in H3. unfold mem_add_acc in H3.
+             destruct (valid_dec m2 b2).
+             contradict v. clear - ineq. unfold Mem.valid_block. xomega.
+             exists (b2 - Mem.nextblock m2)%positive, 0.
+             split. unfold add_inj.
+             rewrite jNone.
+             unfold shiftT, filter_id. rewrite lmap'.
+             replace (b2 - Mem.nextblock m2 + Mem.nextblock m2)%positive with b2; auto. 
+             symmetry; apply Pos.sub_add; xomega.
+             destruct (source j12' m1' b2 delta) eqn:sour; try solve [inversion H3]. destruct p.
+             replace (delta - 0) with delta by omega; auto.
+             symmetry in sour; apply source_SomeE in sour.
+             destruct sour as [b1 [delta' [ofs1 [invertible [leq [mapj [mperm ofs_add]]]]]]].
+             inversion invertible; subst delta b z. 
+             subst j12'. 
+             unfold as_inj, join in mapj. rewrite ext_change_ext in mapj.
+             admit. (*is external and b2 > nextblock m2... must be mapped by l shifted*)
+         + unfold pure_composition_block.
+           inversion Heqoutput.
+           subst j' k'.
+           intros.
+           unfold add_inj in H.
+           destruct (k b2) eqn:kmap.
+           - destruct p. inversion H. subst b z. 
+             rewrite Heqk in kmap. 
+             apply Pure in kmap; destruct kmap as [b1 [ofs12 jmap]].
+             exists b1, ofs12.
+             unfold add_inj. subst j; rewrite jmap; auto.
+           - apply shiftS_Some in H; destruct H as [ineq lmap'].
+             apply pure_filter_Some in lmap'; destruct lmap' as [jNone lmap'].
+             exists (b2 - Mem.nextblock m2)%positive, 0.
+             unfold add_inj.
+             rewrite jNone.
+             unfold shiftT, filter_id. rewrite lmap'.
+             replace (b2 - Mem.nextblock m2 + Mem.nextblock m2)%positive with b2; auto. 
+             symmetry; apply Pos.sub_add; xomega.
+       }
+       
+       (* SM_wd 12 *)
+       assert (SMWD12': SM_wd nu12').
+       { subst nu12'. eapply MKI_wd12; eauto.
+         + subst extS12. intros.
+           destruct (locBlocksSrc nu12 b) eqn:locBS12; auto.
+           right. destruct ExtIncr as [? [? [extS [? [locS ?]]]]].
+           simpl in locS; rewrite locS in locBS12.
+           destruct WDnu'. destruct (disjoint_extern_local_Src b) as [locFalse | extFalse].
+           rewrite locBS12 in locFalse; inversion locFalse.
+           exact extFalse.
+         + subst extT12. intros.
+           destruct (locBlocksTgt nu12 b) eqn:locBT12; auto.
+           right. 
+           unfold bconcat, buni, bshift.
+           destruct ExtIncr as [? [? [extS [? [locS [locT ?]]]]]].
+           destruct SMWD12. destruct (disjoint_extern_local_Tgt b) as [locFalse | extFalse].
+           rewrite locBT12 in locFalse; inversion locFalse.
+           rewrite extFalse; simpl.
+           destruct SMV12 as [DOM12 RNG12].
+           subst sizeM2;
+             rewrite RNG12; auto.
+           unfold RNG, DomTgt.
+           rewrite locBT12; auto.
+         + inversion Heqoutput. unfold add_inj, shiftT; intros.
+           destruct (j b1) eqn:jb1. 
+         - rewrite H in jb1. subst j.
+           destruct SMWD12. apply extern_DomRng in jb1. destruct jb1 as [extS12true extT12true].
+           subst extS12 extT12. apply ExtIncr in extS12true.
+           rewrite extS12true; split; trivial.
+           apply bconcat_larger1; auto.
+         - unfold filter_id in H. destruct (l' b1) eqn:lb1; inversion H.
+           subst extS12 extT12. subst l'.
+           destruct WDnu', p;
+             apply extern_DomRng in lb1.
+           destruct lb1 as [extStrue extTtrue].
+           split; auto.
+           subst sizeM2; apply bconcat_larger2; auto.
+           + intros. subst extT12. apply bconcat_larger1; auto.
+             apply SMWD12 in H.
+             exact H.
+       }
+
+       
+       (* SM_wd 23 *)
+       assert (SMWD23': SM_wd nu23').
+       { subst nu23'; eapply MKI_wd23; eauto.
+         + subst extS23; intros.
+           destruct (locBlocksSrc nu23 b) eqn:locBS23; auto.
+           right. 
+           unfold bconcat, buni, bshift.
+             destruct SMWD23; destruct (disjoint_extern_local_Src b) as [locSfalse | extSfalse].
+           rewrite locBS23 in locSfalse; inversion locSfalse.
+           rewrite extSfalse; simpl.
+           destruct ExtIncr as [? [? [extS [extT [locS [locT ?]]]]]].
+           destruct SMV23 as [DOM23 RNG23].
+           subst sizeM2; rewrite DOM23; auto.
+           unfold DOM, DomSrc. rewrite locBS23; auto.
+         + subst extT23. intros.
+           destruct (locBlocksTgt nu23 b) eqn:locBT23; auto.
+           right. destruct ExtIncr as [? [? [extS [? [locS [locT ?]]]]]].
+           simpl in locT; rewrite locT in locBT23.
+           destruct WDnu'. destruct (disjoint_extern_local_Tgt b) as [locFalse | extFalse].
+           rewrite locBT23 in locFalse; inversion locFalse.
+           exact extFalse.
+         + inversion Heqoutput. unfold add_inj, shiftS; intros.
+           destruct (k b1) eqn:kb1. 
+         - rewrite H in kb1. subst k.
+           destruct SMWD23. apply extern_DomRng in kb1. destruct kb1 as [extS23true extT23true].
+           subst extS23 extT23. destruct ExtIncr as [? [? [extS [extT [locS [locT ?]]]]]].
+           simpl in extT; apply extT in extT23true.
+           rewrite extT23true; split; trivial.
+           apply bconcat_larger1; auto.
+         - rename H into lb1. inversion lb1.
+           destruct ((b1 ?= Mem.nextblock m2)%positive) eqn:ineq; try solve [inversion H2].
+           subst extS23 extT23. subst l'.
+           destruct WDnu'.
+           apply pure_filter_Some in lb1; destruct lb1 as [jmap lb1].
+           apply extern_DomRng in lb1.
+           destruct lb1 as [extStrue extTtrue].
+           split; auto.             
+           replace b1 with ((b1 - sizeM2) + sizeM2)%positive; 
+             subst sizeM2. apply bconcat_larger2; auto.
+           apply Pos.sub_add; destruct (Pos.compare_gt_iff b1 (Mem.nextblock m2)). 
+           apply H; auto.
+           + intros. subst extT23. destruct ExtIncr as [? [? [extS [extT [locS [locT ?]]]]]].
+             apply extT; simpl; auto.
+             apply SMWD23 in H; auto.
+       }
+
+       (****************************
+        * Proving each condition   *
+        ****************************)
+
+       split.
+       (*Compose_sm*)
+       { exact compose. } 
+       split.
+       (* extern_incr12 *)
+       { exact ExtIncr12. }
+       split.
+       (* extern_incr23 *)
+       { exact ExtIncr23. }
+       split.
+       (* pure compositoin *)
+       { exact Pure'. }
+       split.
+       (* Mem.inject 12*)
+       { constructor.
+         + constructor.
+         - { intros b1 b2 delta ofs k0 per H H0. subst m2'.
+             unfold Mem.perm; rewrite (mem_add_accx nu12 nu23 j12' m1 m1' m2); unfold mem_add_acc.
+             (* New trying things*)
+             unfold as_inj in H; apply joinD_Some in H; destruct H as [extmap | [extNone locmap]].
+             + subst nu12'; rewrite ext_change_ext in extmap.
+               
+
+               (*assert (locF: locBlocksSrc nu23 b2 = false) by admit.*)
+               eapply MKI_Some12 in extmap; eauto. 
+               destruct extmap as [jmap | [jmap [b2' [d' [lmap' [b2eq deltaeq]]]]]].
+             - assert (Mem.valid_block m2 b2) by (subst j; auto_sm).
+               destruct (valid_dec m2 b2); try solve[contradict n; auto].
+               assert (locF: locBlocksSrc nu23 b2 = false).
+               { destruct GlueInv as [loc rest]; rewrite <- loc.
+                 subst j; auto_sm. }
+               rewrite locF.
+               erewrite source_SomeI. apply H0.
+               * apply MInj12.
+               * unfold as_inj, join. 
+                 subst j. rewrite jmap; auto.
+               * eapply Fwd1.
+                 subst j; auto_sm.
+                 eapply any_Max_Nonempty; eauto. 
+             - destruct (valid_dec m2 b2); (*first discharge the impossible case*)
+               try solve[subst b2; contradict v; unfold Mem.valid_block; xomega].
+               subst b2 delta. 
+               erewrite (source_SomeI j12' m1' ).
+               eapply H0.
+               
+               admit. (*proven elswhere*)
+               subst j12'.
+               unfold as_inj, join. rewrite ext_change_ext, loc_change_ext.
+               assert (j' b1 = Some ((b1 + Mem.nextblock m2)%positive , 0)) by admit.
+               rewrite H. auto.
+                 eapply any_Max_Nonempty; eauto. 
+             + subst nu12'; rewrite loc_change_ext in locmap.
+               assert (locTrue: locBlocksSrc nu23 b2 = true).
+               { destruct GlueInv as [loc rest]; rewrite <- loc; auto_sm. }
+               rewrite locTrue.
+               rewrite ext_change_ext in extNone.
+               assert (Mem.valid_block m2 b2).
+               { apply SMV12. unfold RNG, DomTgt. apply SMWD12 in locmap. 
+                 destruct locmap as [locS locT]; rewrite locT; apply orb_true_l. }
+               destruct (valid_dec m2 b2); try solve[contradict n; auto].
+
+                (*prove that (k b2 = None) by contradiction*)
+                 destruct (k b2) eqn: kmap. subst k.
+                 { destruct p; apply Pure in kmap.
+                   destruct kmap as [b1' [ofs12 extmap12]].
+                   contradict extmap12. intros HH. auto_sm.
+                 }
+                 destruct ( pubBlocksSrc nu23 b2) eqn:pub23.
+                 erewrite (source_SomeI (local_of nu12) m1); eauto.
+                  destruct (pubBlocksSrc nu12 b1) eqn:pub12.
+                 auto.
+
+                 (* pubBlocksSrc nu23 b2 = true & pubBlocksSrc nu12 b1 = false *)
+                  assert (Permb1: Mem.perm m1 b1 ofs k0 per).
+                 { eapply UnchPrivSrc; eauto;
+                   unfold compose_sm; simpl; apply SMWD12 in locmap; destruct locmap; auto.
+                   eapply SMV12. unfold DOM, DomSrc. rewrite H1; auto. }
+                 eapply MInj12; eauto.
+                 auto_sm. (*local mapped*)
+                 eapply (meminj_no_overlap_inject_incr (as_inj nu12)).
+                 apply MInj12.
+                 apply local_in_all; auto.
+                 { apply Fwd1. 
+                 eapply SMV12; apply SMWD12 in locmap; 
+                 destruct locmap; auto; unfold DOM, DomSrc.
+                 rewrite H1; auto.  eapply any_Max_Nonempty; eauto. }
+                 
+                 (* pubBlocksSrc nu23 b2 = false & "pubBlocksSrc nu12 b1 = false"/proved *)
+                 destruct (pubBlocksSrc nu12 b1) eqn:pub12.
+                 { (*this case yields contradiction*)
+                   apply SMWD12 in pub12. destruct pub12 as [b2' [z [loc12 pubTgt]]].
+                   rewrite locmap in loc12; inversion loc12; subst b2' z.
+                   apply GlueInv in pubTgt.
+                   rewrite pubTgt in pub23; discriminate pub23. }
+                  assert (Permb1: Mem.perm m1 b1 ofs k0 per).
+                 { eapply UnchPrivSrc; eauto;
+                   unfold compose_sm; simpl; apply SMWD12 in locmap; destruct locmap; auto.
+                   eapply SMV12. unfold DOM, DomSrc. rewrite H1; auto. }
+                 eapply MInj12; eauto.
+                 admit.
+                 }
+         - intros. unfold Z.divide.
+           subst nu12'; unfold as_inj, join in H. rewrite ext_change_ext, loc_change_ext in H.
+           destruct (j' b1) eqn:jmap'. 
+           destruct p0. destruct (MKI_Some12 _ _ _ _ _ _ Heqoutput _ _ _ jmap') as 
+                          [jmap | [jmap [b2' [d' [lmap [b2eq deq]]]]]].
+           inversion H; subst b z.
+           subst j. destruct MInj12. destruct mi_inj.
+           eapply (mi_align b1 b2); eauto. 
+           unfold as_inj, join; rewrite jmap; trivial.
+           Lemma forward_range:
+             forall m m' b ofs size p,
+               mem_forward m m' ->
+               Mem.valid_block m b ->
+               Mem.range_perm m' b ofs (ofs + size) Max p ->
+               Mem.range_perm m b ofs (ofs + size) Max p.
+             unfold Mem.range_perm; intros.
+             apply H; auto.
+           Qed.
+           eapply forward_range; eauto.
+           clear H. 
+           Lemma mapped_valid: forall mu m1 m2 b1 b2 d,
+                                 SM_wd mu ->
+                                 as_inj mu b1 = Some (b2, d) ->
+                                 sm_valid mu m1 m2 ->
+                                 Mem.valid_block m1 b1.
+             intros. destruct H1 as [H1 H2]; apply H1.
+             unfold DOM, DomSrc.
+             apply joinD_Some in H0; destruct H0 as [map | [extNone map]];
+             apply H in map; destruct map as [src tgt]; rewrite src; auto.
+             apply orb_true_r.
+           Qed.
+           eapply mapped_valid.
+           apply SMWD12. 
+           unfold as_inj, join; rewrite jmap; auto. 
+           eauto.
+           
+           (* This should be folded in a lemma *)
+           inversion Heqoutput.
+           unfold add_inj, shiftT in H2. subst j'. rewrite jmap in jmap'.
+           unfold filter_id in jmap'. rewrite lmap in jmap'.
+           inversion jmap'. subst z. symmetry in H; inversion H; subst delta.
+           exists 0; xomega.
+           (*Done *)
+           
+           destruct MInj12. destruct mi_inj.
+           eapply (mi_align b1 b2); eauto.
+           unfold as_inj. 
+           rewrite join_com. 
+           unfold join; rewrite H; trivial.
+           apply disjoint_extern_local.
+           apply SMWD12.
+           eapply forward_range; eauto.
+           eapply mapped_valid.
+           apply SMWD12. 
+           unfold as_inj. 
+           rewrite join_com. 
+           unfold join; rewrite H; trivial.
+           apply disjoint_extern_local.
+           apply SMWD12.
+           eauto.
+         - (*TRYING SOMETHING*)
+           { (*intros b1 ofs b2 delta map12' mperm1'.
+             rewrite (mem_add_contx nu12 nu23 j12' m1 m1' m2); unfold mem_add_cont.
+             (* New trying things*)
+             unfold as_inj in map12'; apply joinD_Some in map12'; 
+             destruct map12' as [extmap | [extNone locmap]].
+             + subst nu12'; rewrite ext_change_ext in extmap.
+               assert (locF: locBlocksSrc nu23 b2 = false) by admit.
+               rewrite locF.
+               eapply MKI_Some12 in extmap; eauto. 
+               destruct extmap as [jmap | [jmap [b2' [d' [lmap' [b2eq deltaeq]]]]]].
+             - assert (Mem.valid_block m2 b2).
+               { apply SMV12. unfold RNG, DomTgt. subst j; apply SMWD12 in jmap. 
+                 destruct jmap as [extS extT]; rewrite extT; apply orb_true_r. }
+               destruct (valid_dec m2 b2); try solve[contradict n; auto].
+               erewrite source_SomeI. instantiate(1:= b1).
+               destruct (ZMap.get ofs (Mem.mem_contents m1') !! b1) eqn:theval;
+                 try constructor.
+               unfold inject_memval. 
+               erewrite local_in_all; eauto.
+               econstructor; eauto.
+               unfold as_inj, join; rewrite ext_change_ext, loc_change_ext.
+               rewrite (MKI_incr12 _ _ _ _ _ _ Heqoutput).
+               destruct (as_inj nu12 b). 
+               unfold inject_memval.
+               
+               apply H0.
+               * apply MInj12.
+               * unfold as_inj, join. 
+                 subst j. rewrite jmap; auto.
+               * eapply Fwd1.
+                 admit. (*Mapped by j*)
+                 eapply any_Max_Nonempty; eauto. 
+             - destruct (valid_dec m2 b2); (*first discharge the impossible case*)
+               try solve[subst b2; contradict v; unfold Mem.valid_block; xomega].
+               subst b2 delta. 
+               erewrite (source_SomeI j12' m1' ).
+               eapply H0.
+               admit. (*proven elswhere*)
+               subst j12'.
+               unfold as_inj, join. rewrite ext_change_ext, loc_change_ext.
+               assert (j' b1 = Some ((b1 + Mem.nextblock m2)%positive , 0)) by admit.
+               rewrite H. auto.
+                 eapply any_Max_Nonempty; eauto. 
+             + subst nu12'; rewrite loc_change_ext in locmap.
+               assert (locTrue: locBlocksSrc nu23 b2 = true) by admit.
+               rewrite locTrue.
+               rewrite ext_change_ext in extNone.
+               assert (Mem.valid_block m2 b2).
+               { apply SMV12. unfold RNG, DomTgt. apply SMWD12 in locmap. 
+                 destruct locmap as [locS locT]; rewrite locT; apply orb_true_l. }
+               destruct (valid_dec m2 b2); try solve[contradict n; auto].
+
+                (*prove that (k b2 = None) by contradiction*)
+                 destruct (k b2) eqn: kmap. subst k.
+                 { destruct p; apply Pure in kmap.
+                   destruct kmap as [b1' [ofs12 extmap12]].
+                   admit. (* local and ext map to the same block => contradiction *) }
+                 destruct ( pubBlocksSrc nu23 b2) eqn:pub23.
+                 erewrite (source_SomeI (local_of nu12) m1); eauto.
+                  destruct (pubBlocksSrc nu12 b1) eqn:pub12.
+                 auto.
+
+                 (* pubBlocksSrc nu23 b2 = true & pubBlocksSrc nu12 b1 = false *)
+                  assert (Permb1: Mem.perm m1 b1 ofs k0 per).
+                 { eapply UnchPrivSrc; eauto;
+                   unfold compose_sm; simpl; apply SMWD12 in locmap; destruct locmap; auto.
+                   eapply SMV12. unfold DOM, DomSrc. rewrite H1; auto. }
+                 eapply MInj12; eauto.
+                 admit. (*local mapped*)
+                 admit. (*proved elsewhere*)
+                 { apply Fwd1. 
+                 eapply SMV12; apply SMWD12 in locmap; destruct locmap; auto; unfold DOM, DomSrc.
+                 rewrite H1; auto.
+                 eapply any_Max_Nonempty; eauto. }
+                 
+                 (* pubBlocksSrc nu23 b2 = false & "pubBlocksSrc nu12 b1 = false"/proved *)
+                 destruct (pubBlocksSrc nu12 b1) eqn:pub12.
+                 { (*this case yields contradiction*)
+                   apply SMWD12 in pub12. destruct pub12 as [b2' [z [loc12 pubTgt]]].
+                   rewrite locmap in loc12; inversion loc12; subst b2' z.
+                   apply GlueInv in pubTgt.
+                   rewrite pubTgt in pub23; discriminate pub23. }
+                  assert (Permb1: Mem.perm m1 b1 ofs k0 per).
+                 { eapply UnchPrivSrc; eauto;
+                   unfold compose_sm; simpl; apply SMWD12 in locmap; destruct locmap; auto.
+                   eapply SMV12. unfold DOM, DomSrc. rewrite H1; auto. }
+                 eapply MInj12; eauto.
+                 admit.
+                 }
+
+
+
+unfold as_inj in map12'; apply joinD_Some in map12'; destruct map12' as [extmap | [extNone locmap]].
+             + subst nu12'; rewrite ext_change_ext in extmap.
+               unfold as_inj, join; rewrite ext_change_ext, loc_change_ext.
+               assert (extmap2:=extmap).
+               eapply MKI_Some12 in extmap2; eauto. 
+               destruct extmap2 as [jmap | [jmap [b2' [d' [lmap' [b2eq deltaeq]]]]]].
+             - assert (Mem.valid_block m2 b2).
+               { apply SMV12. unfold RNG, DomTgt. subst j; apply SMWD12 in jmap. 
+                 destruct jmap as [extS extT]; rewrite extT; apply orb_true_r. }
+               destruct (valid_dec m2 b2); try solve[contradict n; auto].
+               erewrite source_SomeI.
+               (* Here is were the proof gets harder than just the perm.*)
+               destruct MemInjNu'. destruct mi_inj.
+               (*Prepare to use mi_memval of nu'*)
+               assert (map13': exists b3 d3, as_inj nu' b1 = Some (b3, d3)).
+               {assert (kmap:=jmap).
+               apply Norm12 in kmap; destruct kmap as [b3 [d2 kmap]].
+               exists b3, (delta + d2).
+               unfold as_inj, join. destruct ExtIncr as [ext_incr other_incr]. 
+               erewrite ext_incr; eauto.
+               rewrite compose_sm_extern. subst j.
+               unfold compose_meminj.
+               rewrite jmap.
+               subst k. rewrite kmap; auto.
+               }
+               destruct map13' as [b3 [d3 map13']].
+               apply (mi_memval b1 ofs b3 d3 map13') in mperm1'.
+               instantiate(1:=b1).
+               inversion mperm1'; try constructor.
+               remember ( change_ext nu12 extS12 extT12 j') as nu12'.
+               rewrite compose in H2.
+               unfold as_inj in H2.
+               { (*Two cases, whether b0 is external or local*)
+                 destruct (joinD_Some _ _ _ _ _ H2) as [extcomp | [extcomp loccomp]].
+                 + (* b0 is external*)
+                   rewrite compose_sm_extern in extcomp.
+                   apply compose_meminjD_Some in extcomp.
+                   destruct extcomp as [b1' [ofs1' [ofs' [ext12 [ext23 eq]]]]].
+                   subst nu12'; rewrite ext_change_ext in ext12.
+                   subst jp; unfold inject_memval, join .
+                   subst j12'; unfold as_inj, join; rewrite ext_change_ext.
+                   rewrite ext12.
+                   econstructor; auto.
+                   rewrite ext12.
+                   reflexivity.
+                 + (* b0 is local / need to show it's public!*)
+                   rewrite compose_sm_local in loccomp.
+                   apply compose_meminjD_Some in loccomp.
+                   destruct loccomp as [b1' [ofs1' [ofs' [loc12 [loc23 eq]]]]].
+                   subst nu12'. rewrite loc_change_ext in loc12.
+                   (* Now let us prove that j b0 = None, to prove jp b0 = b1', ofs1'*)
+                   assert (jmap0': j' b0 = None). 
+                   { remember ( change_ext nu12 extS12 extT12 j') as nu12'.
+                     destruct SMWD12'. 
+                     assert (forall b, local_of nu12 b = local_of nu12' b) by
+                     (intros; subst nu12'; rewrite loc_change_ext; auto).
+                     rewrite H4 in loc12.
+                     apply local_DomRng in loc12.
+                     destruct loc12 as [locS' locT'].
+                     destruct (j' b0) eqn:jmap'; auto. destruct p.
+                     assert (forall b, j' b = extern_of nu12' b) by
+                     (intros; subst nu12'; rewrite ext_change_ext; auto).
+                     rewrite H5 in jmap'. apply extern_DomRng in jmap'.
+                     destruct jmap' as [extS' extT'].
+                     destruct (disjoint_extern_local_Src b0) as [locS'' | extS''].
+                     rewrite locS'' in locS'; inversion locS'.
+                     rewrite extS'' in extS'; inversion extS'. }
+                   subst jp; unfold inject_memval, join. 
+                   subst j12'; unfold as_inj, join; rewrite ext_change_ext, loc_change_ext.
+                   rewrite jmap0'. rewrite loc12.
+                   econstructor.
+                   rewrite jmap0'; eauto.
+                   auto. }
+               * eapply meminj_no_overlap_inject_incr.
+                 eapply (no_overlap_forward _ _ _ _ SMV12); eauto.
+                 apply MInj12.
+                 subst jp. apply inject_incr_join.
+                 subst j; apply inject_incr_refl.
+                 eapply inject_incr_trans; [eapply restrict_incr | apply inject_incr_refl].
+                 apply disjoint_extern_local; eauto.
+               *  subst jp; unfold join; rewrite jmap; auto.
+               * eapply any_Max_Nonempty; eauto.
+             - destruct (valid_dec m2 b2); (*first discharge the impossible case*)
+               try solve[subst b2; contradict v; unfold Mem.valid_block; xomega].
+               subst b2 delta. rewrite Pos.add_sub; auto.
+               replace (ofs + 0) with ofs by omega; trivial.
+               unfold inject_memval.
+               
+               destruct MemInjNu'. destruct mi_inj.
+               (*Prepare to use mi_memval of nu'*)
+               assert (map13': exists b3 d3, as_inj nu' b1 = Some (b3, d3)). 
+               { exists b2', d'. unfold as_inj, join.  subst l'.
+                 rewrite lmap'; auto. }
+               destruct map13' as [b3 [d3 map13']].
+               apply (mi_memval b1 ofs b3 d3 map13') in mperm1'.
+               inversion mperm1'; try constructor.
+               remember ( change_ext nu12 extS12 extT12 j') as nu12'.
+               rewrite compose in H1.
+               unfold as_inj in H1.
+               { (*Two cases, whether b0 is external or local*)
+                 destruct (joinD_Some _ _ _ _ _ H1) as [extcomp | [extcomp loccomp]].
+                 + (* b0 is external*)
+                   rewrite compose_sm_extern in extcomp.
+                   apply compose_meminjD_Some in extcomp.
+                   destruct extcomp as [b1' [ofs1' [ofs' [ext12 [ext23 eq]]]]].
+                   subst nu12'; rewrite ext_change_ext in ext12.
+                   subst jp; unfold inject_memval, join .
+                   subst j12'; unfold as_inj, join; rewrite ext_change_ext.
+                   rewrite ext12.
+                   econstructor; auto.
+                   rewrite ext12.
+                   reflexivity.
+                 + (* b0 is local / need to show it's public!*)
+                   rewrite compose_sm_local in loccomp.
+                   apply compose_meminjD_Some in loccomp.
+                   destruct loccomp as [b1' [ofs1' [ofs' [loc12 [loc23 eq]]]]].
+                   subst nu12'. rewrite loc_change_ext in loc12.
+                   (* Now let us prove that j b0 = None, to prove jp b0 = b1', ofs1'*)
+                   assert (jmap0': j' b0 = None). 
+                   {  remember ( change_ext nu12 extS12 extT12 j') as nu12'.
+                     destruct SMWD12'. 
+                     assert (forall b, local_of nu12 b = local_of nu12' b) by
+                     (intros; subst nu12'; rewrite loc_change_ext; auto).
+                     rewrite H3 in loc12.
+                     apply local_DomRng in loc12.
+                     destruct loc12 as [locS' locT'].
+                     destruct (j' b0) eqn:jmap'; auto. destruct p.
+                     assert (forall b, j' b = extern_of nu12' b) by
+                     (intros; subst nu12'; rewrite ext_change_ext; auto).
+                     rewrite H4 in jmap'. apply extern_DomRng in jmap'.
+                     destruct jmap' as [extS' extT'].
+                     destruct (disjoint_extern_local_Src b0) as [locS'' | extS''].
+                     rewrite locS'' in locS'; inversion locS'.
+                     rewrite extS'' in extS'; inversion extS'. }
+                   subst jp; unfold inject_memval, join. 
+                   subst j12'; unfold as_inj, join; rewrite ext_change_ext, loc_change_ext.
+                   rewrite jmap0'. rewrite loc12.
+                   econstructor.
+                   rewrite jmap0'; eauto.
+                   auto. }
+             + subst nu12'; rewrite loc_change_ext in locmap.
+               rewrite ext_change_ext in extNone.
+               assert (Mem.valid_block m2 b2).
+               { apply SMV12. unfold RNG, DomTgt. apply SMWD12 in locmap. 
+                 destruct locmap as [locS locT]; rewrite locT; apply orb_true_l. }
+               destruct (valid_dec m2 b2); try solve[contradict n; auto].
+               destruct (source jp m1' b2 (ofs + delta)) eqn:sour.
+               - destruct p; symmetry in sour.
+                 destruct (source_SomeE _ _ _ _ _ sour) 
+                               as [b1' [delta' [ofs1 [pairs [bval [jpmap [mperm ofss]]]]]]].
+                 assert (jpmap':= jpmap).
+                 inversion pairs; subst b z jp.
+                 (*b2 is local so j can't map to it *)
+                 unfold join in jpmap.
+                 destruct (j b1') eqn:jmap; try destruct p.
+                 {inversion jpmap; subst b z j.
+                 apply SMWD12 in jmap; destruct jmap as [extS extT].
+                 apply SMWD12 in locmap; destruct locmap as [locS locT].
+                 destruct SMWD12. destruct (disjoint_extern_local_Tgt b2) as [LT | ET];
+                 [rewrite LT in locT | rewrite ET in extT]; discriminate. }
+                 (*j b1' = None, So local_of nu12 maps b1' and it's public*)
+                 apply restrictD_Some in jpmap; destruct jpmap as [locmap' pubtrue].
+                 edestruct (no_overlap_no_doublemap (local_of nu12) b1 b1') as 
+                     [b1_eq [ofs_eq d_eq]]; eauto.
+                 { eapply meminj_no_overlap_inject_incr.
+                   eapply no_overlap_forward. 
+                   apply SMV12.
+                   apply SMWD12.
+                   auto.
+                   apply MInj12.
+                   apply local_in_all. apply SMWD12. }
+                 eapply any_Max_Nonempty; eauto.
+                 destruct MemInjNu'. destruct mi_inj.
+                 
+                 assert (map13': exists b3 d3, as_inj nu' b1 = Some (b3, d3)).
+                 { destruct GlueInv as [loc [ext [pub frgn]]]. 
+                   apply SMWD12 in pubtrue; destruct pubtrue as [b2' [z'[ locmapinv' pubT]]].
+                   rewrite locmapinv' in locmap'; inversion locmap'. 
+                   apply pub in pubT. apply SMWD23 in pubT.
+                   destruct pubT as [b3 [z [locmap23 pubT23]]].
+                   exists b3, (z' + z).
+                   unfold as_inj. rewrite join_com.
+                   remember ( change_ext nu12 extS12 extT12 j') as nu12'.
+                   rewrite compose.
+                   rewrite compose_sm_extern, compose_sm_local.
+                   unfold join, compose_meminj.
+                   subst nu12' nu23'; rewrite ext_change_ext, loc_change_ext.
+                   subst b1' ofs1. rewrite locmapinv'. 
+                   rewrite loc_change_ext.
+                   rewrite locmap23; auto.
+                   apply disjoint_extern_local; auto. }
+                 destruct map13' as [b3 [d3 map13']].
+                 apply (mi_memval b1 ofs b3 d3 map13') in mperm1'.
+                 unfold inject_memval. subst b1' ofs.
+                 inversion mperm1'; try constructor.
+                 remember ( change_ext nu12 extS12 extT12 j') as nu12'.
+                 assert (map12': exists b2' d2', j12' b0 = Some (b2', d2')). 
+                 { rewrite compose in H2.
+                   apply compose_sm_as_injD in H2; eauto.
+                   destruct H2 as [b2' [d1 [d2 [map12' [map23' eq]]]]].
+                    exists b2', d1. subst j12'; apply map12'; auto.
+                 }
+                 destruct map12' as [b2' [d2' mapj12']].
+                 rewrite mapj12'. econstructor; auto.
+                 subst j12'; apply mapj12'.
+               - (*Since source is None, but local_of nu12 b1 =Some, it must be private!*)
+                 assert (jpmap: jp b1 = None). (*By contradiction*)
+                 { subst jp.
+                   apply MKI_incr12 in Heqoutput.
+                   apply (inject_incr_inv _ _ Heqoutput) in extNone.
+                   unfold join. rewrite extNone. 
+                   destruct (restrict (local_of nu12) (pubBlocksSrc nu12) b1) eqn:rest_map12; trivial. destruct p.
+                   destruct (restrictD_Some _ _ _ _ _ rest_map12) as [locmap12 pub12].
+                   rewrite locmap in locmap12. inversion locmap12.
+                   subst b z. clear locmap12.
+                   symmetry in sour; eapply source_NoneE in sour.
+                   contradiction sour. eapply any_Max_Nonempty. instantiate(3:=delta).
+                   replace (ofs + delta - delta) with ofs by omega.
+                   eassumption.
+                   destruct SMV12 as [validD validR].
+                   apply (Pos.lt_le_trans _ (Mem.nextblock m1) _).
+                   apply validD. unfold DOM, DomSrc.
+                   apply SMWD12 in locmap. destruct locmap as [loc12 ?].
+                   rewrite loc12; auto.
+                   apply forward_nextblock; trivial.
+                   unfold join; rewrite extNone; auto. }
+                 subst jp. apply joinD_None in jpmap; destruct jpmap as [jmap locmap'].
+                 eapply restrictD_None in locmap'; eauto.
+                 destruct UnchPrivSrc.
+                 rewrite unchanged_on_contents.
+                 destruct MInj12.
+                 destruct mi_inj.
+                 move mi_memval at bottom.
+                 eapply memval_inject_incr.
+                 eapply mi_memval.
+                 (* discharge the remaining subgoals which are easy *)
+                 (* Notice how many of those repeat... *)
+                 { unfold as_inj; rewrite join_com; unfold join.
+                   rewrite locmap; auto.
+                   apply disjoint_extern_local; apply SMWD12. }
+                 { apply unchanged_on_perm.
+                   unfold compose_sm; simpl; split; auto.
+                   apply SMWD12 in locmap. destruct locmap; trivial. 
+                   destruct SMV12 as [validD validR].
+                   apply validD. unfold DOM, DomSrc.
+                   apply SMWD12 in locmap. destruct locmap as [loc12 ?].
+                   rewrite loc12; auto.
+                   trivial.
+                 }
+                 {  apply extern_incr_as_inj; auto.
+                    (* Both subgoals were proven earlier in the theorem *)
+                 }
+                 { unfold compose_sm; simpl; split; auto.
+                   apply SMWD12 in locmap; destruct locmap; auto. }
+                 { apply unchanged_on_perm.
+                   unfold compose_sm; simpl; split; auto.
+                   apply SMWD12 in locmap. destruct locmap; trivial. 
+                   destruct SMV12 as [validD validR].
+                   apply validD. unfold DOM, DomSrc.
+                   apply SMWD12 in locmap. destruct locmap as [loc12 ?].
+                   rewrite loc12; auto.
+                   trivial. }*) admit.
+                 }
+       + intros. unfold as_inj; subst nu12'; rewrite ext_change_ext, loc_change_ext.
+         assert (H0: ~ Mem.valid_block m1 b). 
+         { clear - H Fwd1. unfold not, Mem.valid_block in *.
+           intros; apply H. apply (Pos.lt_le_trans _ _ _ H0).
+           apply forward_nextblock; assumption. }
+         destruct MInj12, MemInjNu'.
+         apply mi_freeblocks in H0; destruct (as_injD_None _ _ H0) as [ext loc].
+         apply mi_freeblocks0 in H; destruct (as_injD_None _ _ H) as [ext' loc'].
+         unfold join.
+         erewrite MKI_None12; eauto; subst j k l'; eauto.
+       + unfold as_inj; subst nu12' m2'.
+         intros b b' delta map; destruct (as_in_SomeE _ _ _ _ map) as [ext | loc].
+         rewrite ext_change_ext in ext. 
+         destruct (MKI_Some12 _ _ _ _ _ _ Heqoutput _ _ _ ext).
+         destruct MInj12.
+         unfold Mem.valid_block; rewrite mem_add_nbx; unfold mem_add_nb.
+         eapply Pos.lt_trans; try eapply (Pos.lt_add_diag_r (Mem.nextblock m2)).
+         apply (mi_mappedblocks b b' delta).
+         unfold as_inj, join; subst j k l'; rewrite H; auto.
+         destruct H as [jmap [b2' [d' [lmap' [eq1 eq2]]]]].
+         destruct MemInjNu'. unfold Mem.valid_block; rewrite mem_add_nbx.
+         unfold mem_add_nb. subst b'.
+         destruct WDnu'.
+         subst l'.
+         apply extern_DomRng in lmap'; destruct lmap' as [extS extT].
+         destruct SMvalNu' as [DOMv RNGv].
+         assert (Plt b m1'.(Mem.nextblock)).
+         apply DOMv. unfold DOM, DomSrc. rewrite extS; apply orb_true_r.
+         xomega.
+
+         unfold Mem.valid_block; rewrite mem_add_nbx.
+         unfold mem_add_nb.
+         rewrite loc_change_ext in loc.
+         destruct SMWD12.
+         apply local_DomRng in loc; destruct loc as [locS locT].
+         destruct SMV12 as [DOMv RNGv].
+         assert (Plt b' m2.(Mem.nextblock)).
+         apply RNGv. unfold RNG, DomTgt. rewrite locT; apply orb_true_l.
+         xomega.
+       + idtac.
+         Lemma no_overlap_asinj: 
+           forall mu m, 
+             SM_wd mu -> 
+             Mem.meminj_no_overlap (extern_of mu) m ->
+             Mem.meminj_no_overlap (local_of mu) m ->
+             Mem.meminj_no_overlap (as_inj mu) m.
+           unfold Mem.meminj_no_overlap.
+           intros mu m SMWD NOO_ext NOO_loc.
+           intros.
+           apply as_in_SomeE in H0.
+           apply as_in_SomeE in H1.
+           destruct H0 as [ext1 | loc1];
+           destruct H1 as [ext2 | loc2].
+           eapply NOO_ext; eauto.
+           destruct SMWD. apply extern_DomRng in ext1; apply local_DomRng in loc2.
+           destruct (peq b1' b2'); auto; subst b1'.
+           destruct loc2; destruct ext1.
+           destruct (disjoint_extern_local_Tgt b2'). 
+           rewrite H6 in H1; inversion H1.
+           rewrite H6 in H5; inversion H5.
+           destruct SMWD. apply extern_DomRng in ext2; apply local_DomRng in loc1.
+           destruct (peq b1' b2'); auto; subst b1'.
+           destruct loc1; destruct ext2.
+           destruct (disjoint_extern_local_Tgt b2'). 
+           rewrite H6 in H1; inversion H1.
+           rewrite H6 in H5; inversion H5.
+           eapply NOO_loc; eauto.
+         Qed.
+         Lemma no_overlap_ext:
+           forall mu m,
+             Mem.meminj_no_overlap (as_inj mu) m ->
+             Mem.meminj_no_overlap (extern_of mu) m.
+           unfold Mem.meminj_no_overlap; intros.
+           eapply H; eauto.
+           unfold as_inj, join; rewrite H1; auto.
+           unfold as_inj, join; rewrite H2; auto.
+         Qed.
+         Lemma no_overlap_loc:
+           forall mu m,
+             SM_wd mu ->
+             Mem.meminj_no_overlap (as_inj mu) m ->
+             Mem.meminj_no_overlap (local_of mu) m.
+           unfold Mem.meminj_no_overlap; intros.
+           eapply H0; eauto.
+           unfold as_inj; rewrite (join_com _ _ (disjoint_extern_local _ H)); unfold join.
+           rewrite H2; auto.
+           unfold as_inj; rewrite (join_com _ _ (disjoint_extern_local _ H)); unfold join.
+           rewrite H3; auto.
+         Qed.
+         apply no_overlap_asinj; auto.
+         subst nu12'; rewrite ext_change_ext.
+         Lemma MKI_no_overlap12:
+           forall j k l sizeM2,
+           forall j' k',
+             (j', k') = mkInjections sizeM2 j k l ->
+             forall m1 m1',
+             Mem.meminj_no_overlap j m1 ->
+             Mem.meminj_no_overlap l m1' ->
+             mem_forward m1 m1' ->
+             (forall b1 b2 d, j b1 = Some (b2, d) -> Mem.valid_block m1 b1) ->
+             (forall b1 b2 d, j b1 = Some (b2, d) -> Plt b2 sizeM2) ->
+             Mem.meminj_no_overlap j' m1'.
+          unfold Mem.meminj_no_overlap; intros.
+          inversion H. subst j'.
+          Lemma add_inj_Some: forall j k b1 b2 d,
+                                (j (+) k) b1 = Some (b2, d) ->
+                                j b1 = Some (b2, d) \/
+                                k b1 = Some (b2, d).
+          unfold add_inj; intros. destruct (j b1).
+          + destruct p; left; auto.
+          + right; auto.
+          Qed.
+          apply add_inj_Some in H6; destruct H6 as [jmap1 | lmap1];
+          apply add_inj_Some in H7; destruct H7 as [jmap2 | lmap2].
+          (*1: Good case*)
+          + eapply H0; eauto.
+            - assert (Mem.valid_block m1 b1) by (eapply H3; eauto).
+              eapply H2 in H6. destruct H6 as [Memval mperm].
+              apply mperm; auto.
+            - assert (Mem.valid_block m1 b2) by (eapply H3; eauto).
+              eapply H2 in H6. destruct H6 as [Memval mperm].
+              apply mperm; auto.
+          (*2: Bad case/ contradiction*)
+          + apply H4 in jmap1.
+            unfold shiftT in lmap2. destruct ( filter_id l b2); try solve[inversion lmap2].
+            destruct p. inversion lmap2.
+            left. unfold not; intros.
+            subst b1'. contradict jmap1. xomega.
+          (*3: Bad case/ contradiction*)
+          + apply H4 in jmap2.
+            unfold shiftT in lmap1. destruct ( filter_id l b1); try solve[inversion lmap1].
+            destruct p. inversion lmap1.
+            left. unfold not; intros.
+            subst b2'. contradict jmap2. xomega.
+          (*4: Good case/ lmap*)
+          + unfold shiftT in *.
+            unfold filter_id in *.
+            destruct (l b1) eqn:lmap1'; try solve [inversion lmap1]. destruct p.
+            destruct (l b2) eqn:lmap2'; try solve [inversion lmap2]. destruct p.
+            destruct (H1 _ _ _ _ _ _ _ _ H5 lmap1' lmap2' H8 H9) as [ineq1 | ineq2].
+            - inversion lmap1; inversion lmap2. subst.
+              left; clear - H5. unfold not; intros. 
+              apply H5. eapply Pos.add_reg_r; eauto.
+            - inversion lmap1; inversion lmap2. subst.
+              left; clear - H5. unfold not; intros. 
+              apply H5. eapply Pos.add_reg_r; eauto.
+          Qed.
+         (*Mem.meminj_no_overlap j' m1'*)
+         { eapply MKI_no_overlap12; eauto.
+         - subst j. apply no_overlap_ext.
+           apply MInj12.
+         - subst l'; apply no_overlap_ext; eapply MemInjNu'.
+         - intros. apply SMV12. unfold DOM, DomSrc. subst j; apply SMWD12 in H.
+           destruct H as [extS extT]; rewrite extS; apply orb_true_r.
+         - intros. apply SMV12. unfold RNG, DomTgt. subst j; apply SMWD12 in H.
+           destruct H as [extS extT]; rewrite extT; apply orb_true_r. }
+         (*Mem.meminj_no_overlap (local_of nu12') m1'*)
+         { subst nu12'; rewrite loc_change_ext.
+           eapply no_overlap_loc; eauto.
+           eapply no_overlap_forward; eauto.
+           apply MInj12. }
+       + intros.
+         subst nu12'. apply as_in_SomeE in H; destruct H as [ext1 | loc1];
+         [ rewrite ext_change_ext in ext1 | rewrite loc_change_ext in loc1].
+         - eapply MKI_Some12 in ext1; eauto. 
+           destruct ext1 as [jmap | [jmap [b3 [d [lmap' [beq deq]]]]]].
+           assert (map12: as_inj nu12 b = Some (b', delta)).
+           { unfold as_inj, join ; subst j; rewrite jmap; eauto. }
+           destruct MInj12. eapply mi_representable; eauto. 
+           destruct H0; [left | right].
+           eapply Fwd1.
+           Lemma valid_from_map: 
+             forall mu m1 m2 b1 b2 d,
+               SM_wd mu -> 
+               as_inj mu b1 = Some (b2,d) ->
+               sm_valid mu m1 m2 ->
+               Mem.valid_block m1 b1.
+             intros mu m1 m2 b1 b2 d SMWD map smv. 
+             apply as_in_SomeE in map.
+             destruct SMWD, smv as [DOMv RNGv], map as [ext1 | loc1];
+             apply DOMv; unfold DOM, DomSrc.
+             apply extern_DomRng in ext1; destruct ext1 as [extS extT].
+             rewrite extS; apply orb_true_r.
+             apply local_DomRng in loc1; destruct loc1 as [locS locT].
+             rewrite locS; apply orb_true_l.
+             Qed.
+           eapply valid_from_map. 
+           apply SMWD12.
+           apply map12.
+           eassumption.
+           assumption.
+
+           eapply Fwd1.
+           eapply valid_from_map. apply SMWD12.
+           apply map12.
+           eassumption.
+           assumption.
+
+           destruct ofs as [ofs range].
+           subst delta; split; simpl. 
+           xomega. 
+           split.
+           xomega.
+           unfold Int.max_unsigned.
+           xomega.
+         - assert (map12: as_inj nu12 b = Some (b', delta)).
+           { apply local_in_all; auto. }
+           destruct MInj12. eapply mi_representable; eauto. 
+           destruct H0; [left | right].
+           eapply Fwd1; eauto.
+           eapply (valid_from_map nu12); eauto.
+           eapply Fwd1; eauto.
+           eapply (valid_from_map nu12); eauto.
+           }
+       split.
+       (* mem_forward *)
+       { exact Fwd2. }
+       split.
+       (* Mem.inject 23*)
+       { subst m2'; constructor.
+         + constructor.
+         - { intros b1 b2 delta ofs k0 p map23.
+             unfold Mem.perm. rewrite (mem_add_accx nu12 nu23 j12' m1 m1' m2); unfold mem_add_acc.
+             unfold as_inj in map23; apply joinD_Some in map23.
+             destruct map23 as [extmap | [extmap locmap]].
+             + subst nu23'.
+               rewrite ext_change_ext in extmap.
+               eapply MKI_Some23 in extmap; eauto. 
+               destruct extmap as [kmap | [kmap [lmap' bGt]]].
+               - assert (bavl: Mem.valid_block m2 b1).
+                 { apply SMV23; eauto. 
+                   unfold DOM; eapply as_inj_DomRng; eauto.
+                   apply extern_in_all; subst k; eauto. }
+                 destruct (valid_dec m2 b1); try solve[contradict n; auto].
+                 
+                 assert (locS: locBlocksSrc nu23 b1 = false) by (subst k; auto_sm).
+                 rewrite locS.
+                 destruct (source (as_inj nu12) m1 b1 ofs) eqn:sour.
+                 * symmetry in sour. destruct (source_SomeE _ _ _ _ _ sour) 
+                    as [b1' [delta' [ofs1 [pairs [bval [jpmap [mperm ofss]]]]]]].
+                   subst ofs p0. 
+                   replace (ofs1 + delta' + delta) with (ofs1 + (delta' + delta)) by omega.
+                   eapply MemInjNu'.
+                   admit.
+                 * subst k; rewrite (extern_in_all _ _ _ _ kmap).
+                   intros H; inversion H.
+               - assert (bval: ~ Mem.valid_block m2 b1).
+                 { unfold Mem.valid_block.
+                   admit. }
+                 destruct (valid_dec m2 b1); try solve [contradict bval; trivial].
+                 destruct (source j12' m1' b1 ofs) eqn:sour; try solve[intros H; inversion H].
+                 symmetry in sour. destruct (source_SomeE _ _ _ _ _ sour) 
+                                   as [b1' [delta' [ofs1 [pairs [bval' [jpmap [mperm ofss]]]]]]].
+                 subst ofs p0.
+                 replace (ofs1 + delta' + delta) with (ofs1 + (delta' + delta)) by omega.
+                 eapply MemInjNu'.
+                 admit.
+             + subst nu23' ; rewrite loc_change_ext in locmap.
+               assert (bavl: Mem.valid_block m2 b1).
+               { apply SMV23; eauto. 
+                 unfold DOM; eapply as_inj_DomRng; eauto.
+                 apply local_in_all; eauto. }
+               destruct (valid_dec m2 b1); try solve [contradict n; trivial].
+               assert (locS: locBlocksSrc nu23 b1 = true) by auto_sm.
+               rewrite locS.
+               destruct (pubBlocksSrc nu23 b1) eqn:pubS.
+               - destruct (source (local_of nu12) m1 b1 ofs) eqn:sour.
+                 
+                 *  symmetry in sour. destruct (source_SomeE _ _ _ _ _ sour) 
+                                     as [b1' [delta' [ofs1 [pairs [bval' [jpmap [mper ofss]]]]]]].
+                   inversion pairs; subst ofs p0; clear sour.
+                   replace (ofs1 + delta' + delta) with (ofs1 + (delta' + delta)) by omega.
+                   destruct (pubBlocksSrc nu12 b1') eqn: pubS12.
+                   intros mperm. eapply MemInjNu'.
+                   apply local_in_all; auto. rewrite compose; unfold compose_sm; simpl.
+                   rewrite loc_change_ext; unfold compose_meminj.
+                   instantiate(1:=b1').
+                   (*Attention*)
+                   (*This thing behaeve weirdly! check what happens if you don't instantiate...*)
+                   assert (locmap12': local_of nu12' b1' = Some (b1, delta')).
+                   { move ExtIncr12 at bottom; unfold extern_incr in ExtIncr12.
+                     destruct ExtIncr12 as [? [loc_inc ?]].
+                     rewrite <- loc_inc; eauto. } 
+                   rewrite locmap12'; rewrite locmap; auto.
+                   assumption.
+
+                   
+                   intros. eapply UnchLOOR13. 
+                   unfold local_out_of_reach; unfold compose_sm; simpl; split.
+                   auto_sm.
+                   intros b0; intros.
+                   destruct (pubBlocksSrc nu12 b0) eqn:pubS12'; try (right; reflexivity).
+                   unfold compose_meminj in H1. 
+                   destruct (local_of nu12 b0) eqn:locmap12; try solve[inversion H1].
+                   destruct p0.
+                   destruct (eq_block b0 b1'); try subst b0.
+                   rewrite pubS12 in pubS12'; discriminate.
+                   left; intros N. 
+                   apply local_in_all in locmap12; trivial.
+                   apply local_in_all in locmap; trivial.
+                   assert (MX: Mem.perm m2 b1 (ofs1 + delta') Max Nonempty).
+                   {eapply Mem.perm_max; eapply Mem.perm_implies. eassumption. apply perm_any_N. }
+                   destruct (Mem.inject_compose _ _ _ _ _ MInj12 MInj23). 
+                   edestruct (mi_no_overlap b0 b2); try eassumption.
+                   { destruct (local_of nu23 b) eqn:loc23; try solve[inversion H1]. 
+                     destruct p0. instantiate (1:=delta0).
+                     inversion H1; subst b3 delta0.
+                     unfold compose_meminj; rewrite locmap12. 
+                     erewrite (local_in_all nu23); eauto. }
+                   instantiate(1:=delta' + delta). 
+                   { instantiate(1:=b2). unfold compose_meminj.
+                      erewrite (local_in_all nu12); eauto. 
+                      rewrite locmap; auto. }
+                   apply H2; auto.
+                   apply H2; omega.
+                   auto_sm.
+                   replace  (ofs1 + (delta' + delta))  with  (ofs1 + delta' + delta) by omega. 
+                   eapply MInj23.
+                   eapply local_in_all; eauto.
+                   auto.
+
+                   
+                 * (*This case is impossible NOT*)
+                   intros.
+                   eapply UnchLOOR13.
+                   unfold local_out_of_reach; unfold compose_sm; simpl; split.
+                   auto_sm.
+                   intros b0; intros.
+                   unfold compose_meminj in H0.
+                   destruct (local_of nu12 b0) eqn:locmap12; try solve [inversion H0].
+                   destruct p0.
+                   destruct (local_of nu23 b) eqn:locmap23; try solve [inversion H0].
+                   destruct p0; inversion H0. subst b2 delta0. clear H0.
+                   
+                   destruct (eq_block b b1); try subst b.
+                   rewrite locmap in locmap23; inversion locmap23; subst delta.
+                   
+                   symmetry in sour; eapply (source_NoneE) in sour; eauto.
+                   destruct (pubBlocksSrc nu12 b0) eqn:pubS12'; try (right; reflexivity).
+                   left.
+                   replace (ofs + z0 - (z + z0)) with (ofs - z) by omega; eauto.
+                   assert (valid:Mem.valid_block m1 b0) by auto_sm; apply valid.
+                   left; intros N. apply local_in_all in locmap12; trivial.
+                   apply (Mem.perm_inject (as_inj nu12) _ _ _ _ _ _ _ _ locmap12 MInj12) in N.            
+                   edestruct (Mem.mi_no_overlap _ _ _ MInj23 b).
+                   exact n.
+                   apply local_in_all; first [exact SMWD23 | exact locmap23].
+                   apply local_in_all; first [exact SMWD23 | exact locmap].
+                   exact N.
+                   eapply any_Max_Nonempty. exact H.
+                   apply H0; trivial.
+                   apply H0; trivial.
+                   omega.
+                   auto_sm.
+                   eapply MInj23. 
+                   apply local_in_all; first [exact SMWD23 | exact locmap].
+                   exact H.
+               -
+               {
+               intros. eapply UnchLOOR23.
+               unfold local_out_of_reach; split.
+               auto_sm.
+               intros bb2; intros.
+               destruct (pubBlocksSrc nu23 bb2) eqn:pubS23; try (right; reflexivity).
+               destruct (eq_block bb2 b1); try subst bb2.
+                 rewrite pubS23 in pubS; discriminate.
+               left; intros N. 
+               apply local_in_all in H0; trivial.
+               apply local_in_all in locmap; trivial.
+                   assert (MX: Mem.perm m2 b1 ofs Max Nonempty).
+                   {eapply Mem.perm_max; eapply Mem.perm_implies. eassumption. apply perm_any_N. }
+                   destruct (Mem.mi_no_overlap _ _ _ MInj23 bb2 _ _ _ _ _ _ _ n H0 locmap N MX).
+                   apply H1; trivial.
+                   apply H1; clear H1. omega.
+                   auto_sm.
+                   eapply MInj23. apply local_in_all; eauto. apply H.
+               }
+             }
+         - intros. unfold Z.divide.
+           subst nu23'; unfold as_inj, join in H. rewrite ext_change_ext, loc_change_ext in H.
+           destruct (k' b1) eqn:kmap'. 
+           * destruct p0. destruct (MKI_Some23 _ _ _ _ _ _ Heqoutput _ _ _ kmap') as 
+                          [kmap | [kmap [ lmap bGt]]].
+           inversion H; subst b z.
+           subst k. destruct MInj23. destruct mi_inj.
+           eapply (mi_align b1 b2); eauto. 
+           unfold as_inj, join; rewrite kmap; trivial.
+           eapply forward_range; eauto.
+           eapply mapped_valid.
+           apply SMWD23. 
+           unfold as_inj, join; rewrite kmap; auto. 
+           eauto.
+
+           unfold Mem.range_perm, Mem.perm in H0.
+           rewrite (mem_add_accx nu12 nu23 j12' m1 m1' m2) in H0; unfold mem_add_acc in H0.
+           destruct (valid_dec m2 b1).
+           { contradict v. unfold not, Mem.valid_block. clear - bGt.
+             unfold Plt, Pos.lt. intros H; rewrite H in bGt; inversion bGt. }
+           
+           
+           (* This should be folded in a lemma *)
+          (* inversion Heqoutput. inversion H; subst b z.
+           unfold add_inj, shiftS in H3. rewrite H3 in kmap'. rewrite kmap in kmap'.
+           destruct (b1 ?= Mem.nextblock m2)%positive; try solve[inversion kmap'].
+           apply pure_filter_Some in kmap'. destruct kmap' as [jmap lmap'].*)
+           inversion H; subst b z. 
+           eapply MemInjNu'.
+           eapply extern_in_all. subst l'. 
+           instantiate(1:=b2). instantiate(1:=(b1 - Mem.nextblock m2)%positive). 
+            exact lmap.
+            unfold Mem.range_perm.
+            intros ofs0 H1. apply H0 in H1.
+            destruct (source j12' m1' b1 ofs0) eqn:sour; try solve [inversion H1].
+
+            
+            symmetry in sour; apply source_SomeE in sour.
+            destruct sour as [b1' [delta' [ofs1 [invertible [leq [mapj [mperm ofs_add]]]]]]].
+            subst p0 ofs0.
+            subst j12'. unfold as_inj, join in mapj. 
+            
+            inversion Heqoutput.
+            subst nu12'. rewrite ext_change_ext in mapj.
+            rewrite H3 in mapj.
+            unfold add_inj in mapj. 
+            destruct ( j b1') eqn:jmap. destruct p0; inversion mapj; subst b1 delta'.
+            {contradict n. 
+            apply SMV12. unfold RNG, DomTgt.
+            subst j. apply SMWD12 in jmap. destruct jmap as [extS extT]; rewrite extT.
+            apply orb_true_r. }
+            unfold filter_id, shiftT in mapj.
+            (*b1, b1' and b2 are externs, so l' must map them, not local_of...*)
+            instantiate(1:=p).
+            admit.
+
+            * unfold Mem.range_perm, Mem.perm in H0.
+              rewrite (mem_add_accx nu12 nu23 j12' m1 m1' m2) in H0; 
+                unfold mem_add_acc in H0.
+              assert (Mem.valid_block m2 b1) by auto_sm.
+              destruct (valid_dec m2 b1); try solve [contradict n; trivial].
+              assert (loc23: locBlocksSrc nu23 b1 = true) by auto_sm.
+              rewrite loc23 in H0.
+              admit.
+           
+           
+         - (*TRYING SOMETHING*)
+           { admit.
+             (*
+               intros b1 ofs b2 delta map12' mperm1'.
+             rewrite (mem_add_contx j12' k jp m1' m2); unfold mem_add_cont.
+             
+             (* New trying things*)
+             unfold as_inj in map12'; apply joinD_Some in map12'; destruct map12' as [extmap | [extNone locmap]].
+             + subst nu12'; rewrite ext_change_ext in extmap.
+               unfold as_inj, join; rewrite ext_change_ext, loc_change_ext.
+               assert (extmap2:=extmap).
+               eapply MKI_Some12 in extmap2; eauto. 
+               destruct extmap2 as [jmap | [jmap [b2' [d' [lmap' [b2eq deltaeq]]]]]].
+             - assert (Mem.valid_block m2 b2).
+               { apply SMV12. unfold RNG, DomTgt. subst j; apply SMWD12 in jmap. 
+                 destruct jmap as [extS extT]; rewrite extT; apply orb_true_r. }
+               destruct (valid_dec m2 b2); try solve[contradict n; auto].
+               erewrite source_SomeI.
+               (* Here is were the proof gets harder than just the perm.*)
+               destruct MemInjNu'. destruct mi_inj.
+               (*Prepare to use mi_memval of nu'*)
+               assert (map13': exists b3 d3, as_inj nu' b1 = Some (b3, d3)).
+               {assert (kmap:=jmap).
+               apply Norm12 in kmap; destruct kmap as [b3 [d2 kmap]].
+               exists b3, (delta + d2).
+               unfold as_inj, join. destruct ExtIncr as [ext_incr other_incr]. 
+               erewrite ext_incr; eauto.
+               rewrite compose_sm_extern. subst j.
+               unfold compose_meminj.
+               rewrite jmap.
+               subst k. rewrite kmap; auto.
+               }
+               destruct map13' as [b3 [d3 map13']].
+               apply (mi_memval b1 ofs b3 d3 map13') in mperm1'.
+               instantiate(1:=b1).
+               inversion mperm1'; try constructor.
+               remember ( change_ext nu12 extS12 extT12 j') as nu12'.
+               rewrite compose in H2.
+               unfold as_inj in H2.
+               { (*Two cases, whether b0 is external or local*)
+                 destruct (joinD_Some _ _ _ _ _ H2) as [extcomp | [extcomp loccomp]].
+                 + (* b0 is external*)
+                   rewrite compose_sm_extern in extcomp.
+                   apply compose_meminjD_Some in extcomp.
+                   destruct extcomp as [b1' [ofs1' [ofs' [ext12 [ext23 eq]]]]].
+                   subst nu12'; rewrite ext_change_ext in ext12.
+                   subst jp; unfold inject_memval, join .
+                   subst j12'; unfold as_inj, join; rewrite ext_change_ext.
+                   rewrite ext12.
+                   econstructor; auto.
+                   rewrite ext12.
+                   reflexivity.
+                 + (* b0 is local / need to show it's public!*)
+                   rewrite compose_sm_local in loccomp.
+                   apply compose_meminjD_Some in loccomp.
+                   destruct loccomp as [b1' [ofs1' [ofs' [loc12 [loc23 eq]]]]].
+                   subst nu12'. rewrite loc_change_ext in loc12.
+                   (* Now let us prove that j b0 = None, to prove jp b0 = b1', ofs1'*)
+                   assert (jmap0': j' b0 = None). 
+                   { remember ( change_ext nu12 extS12 extT12 j') as nu12'.
+                     destruct SMWD12'. 
+                     assert (forall b, local_of nu12 b = local_of nu12' b) by
+                     (intros; subst nu12'; rewrite loc_change_ext; auto).
+                     rewrite H4 in loc12.
+                     apply local_DomRng in loc12.
+                     destruct loc12 as [locS' locT'].
+                     destruct (j' b0) eqn:jmap'; auto. destruct p.
+                     assert (forall b, j' b = extern_of nu12' b) by
+                     (intros; subst nu12'; rewrite ext_change_ext; auto).
+                     rewrite H5 in jmap'. apply extern_DomRng in jmap'.
+                     destruct jmap' as [extS' extT'].
+                     destruct (disjoint_extern_local_Src b0) as [locS'' | extS''].
+                     rewrite locS'' in locS'; inversion locS'.
+                     rewrite extS'' in extS'; inversion extS'. }
+                   subst jp; unfold inject_memval, join. 
+                   subst j12'; unfold as_inj, join; rewrite ext_change_ext, loc_change_ext.
+                   rewrite jmap0'. rewrite loc12.
+                   econstructor.
+                   rewrite jmap0'; eauto.
+                   auto. }
+               * eapply meminj_no_overlap_inject_incr.
+                 eapply (no_overlap_forward _ _ _ _ SMV12); eauto.
+                 apply MInj12.
+                 subst jp. apply inject_incr_join.
+                 subst j; apply inject_incr_refl.
+                 eapply inject_incr_trans; [eapply restrict_incr | apply inject_incr_refl].
+                 apply disjoint_extern_local; eauto.
+               *  subst jp; unfold join; rewrite jmap; auto.
+               * eapply any_Max_Nonempty; eauto.
+             - destruct (valid_dec m2 b2); (*first discharge the impossible case*)
+               try solve[subst b2; contradict v; unfold Mem.valid_block; xomega].
+               subst b2 delta. rewrite Pos.add_sub; auto.
+               replace (ofs + 0) with ofs by omega; trivial.
+               unfold inject_memval.
+               
+               destruct MemInjNu'. destruct mi_inj.
+               (*Prepare to use mi_memval of nu'*)
+               assert (map13': exists b3 d3, as_inj nu' b1 = Some (b3, d3)). 
+               { exists b2', d'. unfold as_inj, join.  subst l'.
+                 rewrite lmap'; auto. }
+               destruct map13' as [b3 [d3 map13']].
+               apply (mi_memval b1 ofs b3 d3 map13') in mperm1'.
+               inversion mperm1'; try constructor.
+               remember ( change_ext nu12 extS12 extT12 j') as nu12'.
+               rewrite compose in H1.
+               unfold as_inj in H1.
+               { (*Two cases, whether b0 is external or local*)
+                 destruct (joinD_Some _ _ _ _ _ H1) as [extcomp | [extcomp loccomp]].
+                 + (* b0 is external*)
+                   rewrite compose_sm_extern in extcomp.
+                   apply compose_meminjD_Some in extcomp.
+                   destruct extcomp as [b1' [ofs1' [ofs' [ext12 [ext23 eq]]]]].
+                   subst nu12'; rewrite ext_change_ext in ext12.
+                   subst jp; unfold inject_memval, join .
+                   subst j12'; unfold as_inj, join; rewrite ext_change_ext.
+                   rewrite ext12.
+                   econstructor; auto.
+                   rewrite ext12.
+                   reflexivity.
+                 + (* b0 is local / need to show it's public!*)
+                   rewrite compose_sm_local in loccomp.
+                   apply compose_meminjD_Some in loccomp.
+                   destruct loccomp as [b1' [ofs1' [ofs' [loc12 [loc23 eq]]]]].
+                   subst nu12'. rewrite loc_change_ext in loc12.
+                   (* Now let us prove that j b0 = None, to prove jp b0 = b1', ofs1'*)
+                   assert (jmap0': j' b0 = None). 
+                   {  remember ( change_ext nu12 extS12 extT12 j') as nu12'.
+                     destruct SMWD12'. 
+                     assert (forall b, local_of nu12 b = local_of nu12' b) by
+                     (intros; subst nu12'; rewrite loc_change_ext; auto).
+                     rewrite H3 in loc12.
+                     apply local_DomRng in loc12.
+                     destruct loc12 as [locS' locT'].
+                     destruct (j' b0) eqn:jmap'; auto. destruct p.
+                     assert (forall b, j' b = extern_of nu12' b) by
+                     (intros; subst nu12'; rewrite ext_change_ext; auto).
+                     rewrite H4 in jmap'. apply extern_DomRng in jmap'.
+                     destruct jmap' as [extS' extT'].
+                     destruct (disjoint_extern_local_Src b0) as [locS'' | extS''].
+                     rewrite locS'' in locS'; inversion locS'.
+                     rewrite extS'' in extS'; inversion extS'. }
+                   subst jp; unfold inject_memval, join. 
+                   subst j12'; unfold as_inj, join; rewrite ext_change_ext, loc_change_ext.
+                   rewrite jmap0'. rewrite loc12.
+                   econstructor.
+                   rewrite jmap0'; eauto.
+                   auto.*) }
+      + intros b H. unfold Mem.valid_block in H.
+        rewrite (mem_add_nbx nu12 nu23 j12' m1 m1' m2) in H.
+        unfold mem_add_nb in H.
+        destruct (as_inj nu23' b) eqn:map; trivial.
+        contradict H. unfold as_inj in map; destruct p.
+        destruct (joinD_Some _ _ _ _ _ map) as [extmap | [extmap locmap]].
+         - subst nu23'. rewrite ext_change_ext in extmap.
+           inversion Heqoutput; subst k'.
+           unfold add_inj in extmap. 
+           destruct (k b) eqn:kmap.
+           assert (Mem.valid_block m2 b).
+           { eapply SMV23. unfold DOM, DomSrc.
+             inversion extmap; subst p k. apply SMWD23 in kmap.
+             destruct kmap as [extS extT]; rewrite extS; apply orb_true_r. }
+           unfold Mem.valid_block in H. apply (Plt_trans _ _ _ H); xomega.
+           apply shiftS_Some in extmap.
+           destruct extmap.
+           apply pure_filter_Some in H1; destruct H1.
+           { assert (Mem.valid_block m1' (b - Mem.nextblock m2)%positive ) 
+               by (subst l'; auto_sm).
+           unfold Mem.valid_block in H3. clear - H H3. 
+           unfold Plt in *. 
+           apply Pos.lt_iff_add; apply Pos.lt_iff_add in H3. destruct H3 as  [r sum].
+           exists r. 
+           rewrite Pos.add_comm in *.
+           rewrite <- sum.
+           rewrite (Pos.add_comm (Mem.nextblock m2) (r + (b - Mem.nextblock m2))).
+           rewrite <- Pos.add_assoc.
+           rewrite Pos.sub_add; eauto.
+           apply Pos.gt_lt_iff; auto. }
+           
+         - assert (Mem.valid_block m2 b).
+           { eapply SMV23. unfold DOM, DomSrc. subst nu23'.
+             rewrite loc_change_ext in locmap.
+             apply SMWD23 in locmap.
+             destruct locmap as [locS locT]; rewrite locS; apply orb_true_l. }
+           unfold Mem.valid_block in H. apply (Plt_trans _ _ _ H); xomega.
+       + intros b b' d H.
+         unfold as_inj. 
+         subst nu23'; destruct (joinD_Some _ _ _ _ _ H) as [extmap | [extmap locmap]].
+         - rewrite ext_change_ext in extmap.
+           inversion Heqoutput; subst k'.
+            unfold add_inj in extmap. 
+            destruct (k b) eqn:kmap.
+           assert (Mem.valid_block m3 b').
+           { eapply SMV23. unfold RNG, DomTgt.
+             inversion extmap; subst p k. apply SMWD23 in kmap.
+             destruct kmap as [extS extT]; rewrite extT; apply orb_true_r. }
+           eapply Fwd3 in H0. destruct H0; auto.
+           apply shiftS_Some in extmap.
+           destruct extmap.
+           apply pure_filter_Some in H2.
+           destruct H2 as [? ?].
+           apply SMvalNu'.
+           unfold RNG, DomTgt.
+           subst l'. apply WDnu' in H3; destruct H3. rewrite H4; apply orb_true_r.
+         - assert (Mem.valid_block m3 b').
+           { eapply SMV23. unfold RNG, DomTgt.
+             rewrite loc_change_ext in locmap.
+             apply SMWD23 in locmap.
+             destruct locmap as [locS locT]; rewrite locT; apply orb_true_l. }
+           eapply Fwd3 in H0. destruct H0; auto.
+       + intros.
+         eapply no_overlap_asinj; auto.
+         - { (*no_overlap extern*)
+             unfold Mem.meminj_no_overlap; intros.
+             subst nu23'. rewrite ext_change_ext in H0, H1.
+             inversion Heqoutput; subst k'.
+             unfold add_inj in H0, H1. 
+             destruct (k b1) eqn:kmap1; destruct (k b2) eqn:kmap2. 
+             (*1. Good case old externs *)
+             eapply MInj23.
+             apply H.
+             eapply extern_in_all; auto.
+             inversion H0; subst k p; trivial.
+             eapply extern_in_all; auto.
+             inversion H1; subst k p0; trivial.
+             apply Fwd2; eauto.
+             subst k; auto_sm.
+             apply Fwd2; eauto.
+             subst k ; auto_sm.
+             (*2.cross case: Dificult case *)
+             { rewrite H0 in kmap1.
+               apply shiftS_Some in H1. destruct H1.
+               apply pure_filter_Some in H4. destruct H4.
+               inversion H0; subst p; clear H0.
+               rewrite Heqk in kmap1.
+               assert(kmap1':=kmap1).
+               unfold Mem.perm in H2, H3.
+               rewrite (mem_add_accx nu12 nu23 j12' m1 m1' m2) in H2, H3; 
+                 unfold mem_add_acc in H2,H3.
+               assert (Mem.valid_block m2 b1) by auto_sm.
+               destruct (valid_dec m2 b1); 
+                 try solve[destruct n; eauto].
+               destruct (valid_dec m2 b2).
+               { (* impossible case. *)
+               move v0 at bottom.
+               unfold Mem.valid_block, Plt, Pos.lt in v0. 
+               unfold Pos.gt in H1. rewrite H1 in v0; inversion v0. }
+               destruct (source j12' m1' b2 ofs2) eqn:sour2; try solve[inversion H3].
+               assert (locF: locBlocksSrc nu23 b1 = false) by auto_sm.
+               rewrite locF in H2.
+               assert (totmap23: as_inj nu23 b1 = Some (b1', delta1)) 
+                 by (apply extern_in_all; trivial).
+               rewrite totmap23 in H2.
+               destruct (source (as_inj nu12) m1 b1 ofs1) eqn:sour1; try solve[inversion H2].
+               symmetry in sour1, sour2. apply source_SomeE in sour1; apply source_SomeE in sour2.
+               destruct sour1 as [b01 [d01 [ofs01 [invert1 [bval1' [map121 [mparm1 of_eq1] ]]]]]].
+               subst p0 ofs1.
+               destruct sour2 as [b02 [d02 [ofs02 [invert2 [bval2' [map122 [mparm2 of_eq2] ]]]]]].
+               subst p ofs2.
+               replace (ofs01 + d01 + delta1) with (ofs01 + (d01 + delta1)) by omega.
+               replace (ofs02 + d02 + delta2) with (ofs02 + (d02 + delta2)) by omega.
+               assert (H': b01<> (b2 - Mem.nextblock m2)%positive).
+               { intros HH; subst b01.
+                 unfold as_inj, join in map121. rewrite Heqj in H4; rewrite H4 in map121.
+                 eapply SMWD12 in map121. destruct map121. destruct GlueInv as [loc rest].
+                 rewrite loc in H8. rewrite locF in H8; inversion H8. }
+               assert (d02 = 0) by admit.
+               assert (b02 = (b2 - Mem.nextblock m2)%positive) by admit.
+               eapply MemInjNu'.
+               apply H'.
+               {
+               subst nu'.
+               unfold as_inj, join.
+               rewrite compose_sm_extern, ext_change_ext.
+               rewrite compose_sm_local, loc_change_ext.
+               subst nu12'. rewrite ext_change_ext, loc_change_ext.
+               assert (jmap11: j b01 = Some (b1, d01)) by admit. 
+               unfold compose_meminj. subst j'. unfold add_inj.
+               rewrite jmap11. subst k. rewrite kmap1. auto. }
+               { (*First show d02 = 0*)
+                 assert (d02 = 0) by admit.
+                 subst d02. replace (0 + delta2) with delta2 by omega.
+                 unfold as_inj, join. 
+                 subst l'; rewrite H6. auto. }
+               auto.
+               subst b02; auto. }
+             (*3.cross case: Dificult case *)
+             { rewrite H1 in kmap2.
+               apply shiftS_Some in H0. destruct H0.
+               apply pure_filter_Some in H4. destruct H4.
+               inversion H1; subst p; clear H1.
+               rewrite Heqk in kmap2.
+               assert(kmap2':=kmap2).
+               unfold Mem.perm in H2, H3.
+               rewrite (mem_add_accx nu12 nu23 j12' m1 m1' m2) in H2, H3; 
+                 unfold mem_add_acc in H2,H3.
+               assert (Mem.valid_block m2 b2) by auto_sm.
+               destruct (valid_dec m2 b2) eqn:bval2; 
+                 try solve[destruct n; eauto].
+               destruct (valid_dec m2 b1) eqn:bval1.
+               { unfold Mem.valid_block, Plt, Pos.lt in v0. move v0 at bottom.
+               unfold Pos.gt in H0. rewrite v0 in H0; inversion H0. }
+               destruct (source j12' m1' b1 ofs1) eqn:sour1; try solve[inversion H2].
+               assert (locF: locBlocksSrc nu23 b2 = false) by auto_sm.
+               rewrite locF in H3.
+               assert (totmap23: as_inj nu23 b2 = Some (b2', delta2)) 
+                 by (apply extern_in_all; trivial).
+               rewrite totmap23 in H3.
+               destruct (source (as_inj nu12) m1 b2 ofs2) eqn:sour2; try solve[inversion H3].
+               symmetry in sour1, sour2. apply source_SomeE in sour1; apply source_SomeE in sour2.
+               destruct sour1 as [b01 [d01 [ofs01 [invert1 [bval1' [map121 [mparm1 of_eq1] ]]]]]].
+               subst p ofs1.
+               destruct sour2 as [b02 [d02 [ofs02 [invert2 [bval2' [map122 [mparm2 of_eq2] ]]]]]].
+               subst p0 ofs2.
+               replace (ofs01 + d01 + delta1) with (ofs01 + (d01 + delta1)) by omega.
+               replace (ofs02 + d02 + delta2) with (ofs02 + (d02 + delta2)) by omega.
+               assert (d01 = 0) by admit.
+               assert (b01 = (b1 - Mem.nextblock m2)%positive) by admit.
+               assert (H': (b1 - Mem.nextblock m2)%positive <> b02) by admit.
+               eapply MemInjNu'.
+               apply H'.
+               { (*First show d01 = 0*)
+                 assert (d01 = 0) by admit.
+                 subst d01. replace (0 + delta1) with delta1 by omega.
+                 unfold as_inj, join. 
+                 subst l'; rewrite H6. auto. }
+               {
+               subst nu'.
+               unfold as_inj, join.
+               rewrite compose_sm_extern, ext_change_ext.
+               rewrite compose_sm_local, loc_change_ext.
+               subst nu12'. rewrite ext_change_ext, loc_change_ext.
+               assert (jmap12: j b02 = Some (b2, d02)) by admit.
+               unfold compose_meminj. subst j'. unfold add_inj.
+               rewrite jmap12. subst k. rewrite kmap2. auto. }
+
+               subst b01; auto. auto.
+             }
+             { (*4. El caso de nu'*)
+               apply shiftS_Some in H0; apply shiftS_Some in H1.
+               destruct H0 as [bval1 pfmap1]; destruct H1 as [bval2 pfmap2].
+               apply pure_filter_Some in pfmap1; apply pure_filter_Some in pfmap2.
+               destruct pfmap1 as [jmpa1 lmap1']; destruct pfmap2 as [jmap2 lmap2'].
+               
+               unfold Mem.perm in H2, H3.
+               rewrite (mem_add_accx nu12 nu23 j12' m1 m1' m2) in H2, H3; 
+                 unfold mem_add_acc in H2,H3.
+               destruct (valid_dec m2 b1).
+               {contradict v. unfold Mem.valid_block. xomega. }
+               destruct (valid_dec m2 b2).
+               {contradict v. unfold Mem.valid_block. xomega. }
+               destruct (source j12' m1' b1 ofs1) eqn:source1; try solve[inversion H2].
+               destruct (source j12' m1' b2 ofs2) eqn:source2; try solve[inversion H3].
+               assert (H': (b1 - Mem.nextblock m2)%positive <> (b2 - Mem.nextblock m2)%positive).
+               { intros eq. apply H. clear - eq bval2 bval1. 
+                 admit. }
+               eapply MemInjNu'.
+               apply H'.
+               unfold as_inj, join. subst l'; rewrite lmap1'; auto.
+               unfold as_inj, join. subst l'; rewrite lmap2'; auto.
+               { (*Use the source luke*)
+                 (*also use Norm!*)
+                 destruct p.
+                 assert (b = (b1 - Mem.nextblock m2)%positive) by admit.
+                 assert (z = ofs1) by admit.
+                 subst b z; auto. }
+               { (*Use the source luke*)
+                 (*also use Norm!*)
+                 destruct p0.
+                 assert (b = (b2 - Mem.nextblock m2)%positive) by admit.
+                 assert (z = ofs2) by admit.
+                 subst b z; auto. }
+               }
+             }
+         - subst nu23'. rewrite loc_change_ext.
+           unfold Mem.meminj_no_overlap; intros.
+           eapply MInj23.
+           apply H.
+           eapply local_in_all; auto.
+           eapply local_in_all; auto.
+           apply Fwd2; eauto.
+           auto_sm.
+           apply Fwd2; eauto.
+           auto_sm.
+       + (*This prove seems identical to the 12 one*)
+         intros.
+         subst nu23'. apply as_in_SomeE in H; destruct H as [ext1 | loc1];
+         [ rewrite ext_change_ext in ext1 | rewrite loc_change_ext in loc1].
+         - eapply MKI_Some23 in ext1; eauto. 
+           destruct ext1 as [kmap | [kmap [lmap bt]]].
+           assert (map23: as_inj nu23 b = Some (b', delta)).
+           { apply extern_in_all; subst k; trivial. }
+           eapply MInj23; eauto.
+           destruct H0; [left | right].
+           eapply Fwd2.
+           eapply valid_from_map. 
+           apply SMWD23.
+           apply map23.
+           eassumption.
+           assumption.
+
+           eapply Fwd2.
+           eapply valid_from_map. apply SMWD23.
+           apply map23.
+           eassumption.
+           assumption.
+
+           eapply MemInjNu'.
+           apply extern_in_all; subst l'; eauto.
+           unfold Mem.perm in H0.
+           rewrite (mem_add_accx nu12 nu23 j12' m1 m1' m2) in H0; 
+                 unfold mem_add_acc in H0.
+           assert (bval: ~Mem.valid_block m2 b). 
+             { unfold Mem.valid_block, Plt, Pos.lt; intros HH. 
+               rewrite bt in HH; inversion HH. }
+           destruct ( valid_dec m2 b); try solve [contradict bval; trivial].
+           destruct H0 as [H | H].
+           * destruct (source j12' m1' b (Int.unsigned ofs)) eqn:sour; 
+             try solve[ inversion H ].
+             left. admit.
+           * destruct (source j12' m1' b (Int.unsigned ofs - 1)) eqn:sour; 
+             try solve[ inversion H ].
+             right. admit.
+         
+         - assert (map23: as_inj nu23 b = Some (b', delta)).
+           { apply local_in_all; auto. }
+           destruct MInj23. eapply mi_representable; eauto. 
+           destruct H0; [left | right].
+           eapply Fwd2; eauto.
+           eapply (valid_from_map nu23); eauto.
+           eapply Fwd2; eauto.
+           eapply (valid_from_map nu23); eauto.
+       }
+       split.
+       (* sm_valid 12'*)
+       { unfold sm_valid.
+         split; intros.
+         apply SMvalNu'. generalize H; unfold DOM, DomSrc.
+         subst nu12'. unfold change_ext; destruct nu12.
+         simpl. rewrite HeqextS12.
+         intros H0.
+         apply orb_true_iff in H0; destruct H0. 
+         destruct ExtIncr as [extincr [intincr [? [? [locS [? [? [? [? ? ]]]]]]]]]; simpl in *.
+         rewrite <- locS. rewrite H0; auto.
+         rewrite H0; apply orb_true_r.
+         
+         (* Valid block *)
+         { subst nu12' m2'. unfold RNG, DomTgt, change_ext in H. destruct nu12; simpl in H.
+           unfold Mem.valid_block. rewrite mem_add_nbx. unfold mem_add_nb.
+           apply orb_true_iff in H; destruct H.
+           + destruct SMV12 as [DOMtrue RNGtrue].
+             unfold RNG, DomTgt in RNGtrue; move RNGtrue at bottom; simpl in RNGtrue.
+             Lemma pos_lt_inc1: forall a b c, (a < b -> a < (b +c ))%positive.
+               intros a b c H.
+               apply Pos.lt_iff_add; apply Pos.lt_iff_add in H.
+               destruct H as [r H].
+               exists (r + c)%positive.
+               rewrite Pos.add_assoc; rewrite H; auto.
+             Qed.
+             apply pos_lt_inc1. apply RNGtrue. rewrite H; auto.
+           + subst extT12; simpl in H.
+             unfold bconcat, buni, bshift in H.
+             apply orb_true_iff in H; destruct H.
+           - destruct SMV23 as [DOMtrue RNGtrue].
+             unfold DOM, DomSrc in DOMtrue; move DOMtrue at bottom; simpl in DOMtrue.
+             apply pos_lt_inc1. apply DOMtrue. 
+             destruct GlueInv as [? [extEq [? ?]]].
+             simpl in extEq. move extEq at bottom. rewrite extEq in H.
+             rewrite H; auto.
+             apply orb_true_r.
+           - destruct ((b2 ?= sizeM2)%positive) eqn:compara; try solve [inversion H].
+             * apply Pos.compare_eq_iff in compara; subst b2.
+               apply Pos.lt_iff_add. exists (Mem.nextblock m1'); subst sizeM2; auto. 
+             * apply Pos.compare_gt_iff in compara.
+               destruct SMvalNu' as [DOMtrue RNGtrue].
+               unfold DOM, DomSrc in DOMtrue; move DOMtrue at bottom; simpl in DOMtrue.
+               specialize (DOMtrue ((b2 - sizeM2)%positive)).
+               rewrite H in DOMtrue. rewrite orb_true_r in DOMtrue.
+               Lemma handy_lemma: forall a b c, (b<a -> a - b < c -> a < b +c )%positive.
+                 intros a b c H1 H2.
+                 destruct (Pos.add_lt_mono_r b (a-b) c) as [HH HH']; apply HH in H2; clear HH HH'.
+                 rewrite (Pos.sub_add a b H1) in H2.
+                 rewrite (Pos.add_comm c b) in H2; assumption.
+               Qed.
+               apply handy_lemma; subst sizeM2; try apply DOMtrue; auto.
+         }
+       }
+       split.
+       (* sm_valid 23'*)
+       { unfold sm_valid.
+         split; intros.
+         subst nu23' m2'. unfold DOM, DomSrc, change_ext in H. destruct nu23; simpl in H.
+         subst extS23; simpl in H.
+         (* Valid block *)
+         { unfold DOM, DomSrc, change_ext in H.
+           unfold Mem.valid_block. rewrite mem_add_nbx. unfold mem_add_nb.
+           apply orb_true_iff in H; destruct H.
+           + destruct SMV23 as [DOMtrue RNGtrue].
+             unfold DOM, DomSrc in DOMtrue; move DOMtrue at bottom; simpl in DOMtrue.
+             apply pos_lt_inc1. apply DOMtrue. rewrite H; auto.
+           + unfold bconcat, buni, bshift in H.
+             apply orb_true_iff in H; destruct H.
+           - destruct SMV12 as [DOMtrue RNGtrue].
+             unfold RNG, DomTgt in RNGtrue; move RNGtrue at bottom; simpl in RNGtrue.
+             apply pos_lt_inc1. apply RNGtrue. 
+             destruct GlueInv as [? [extEq [? ?]]].
+             simpl in extEq. move extEq at bottom. rewrite <- extEq in H.
+             rewrite H; auto.
+             apply orb_true_r.
+           - destruct ((b1 ?= sizeM2)%positive) eqn:compara; try solve [inversion H].
+             * apply Pos.compare_eq_iff in compara; subst b1.
+               apply Pos.lt_iff_add. exists (Mem.nextblock m1'); subst sizeM2; auto. 
+             * apply Pos.compare_gt_iff in compara.
+               destruct SMvalNu' as [DOMtrue RNGtrue].
+               unfold DOM, DomSrc in DOMtrue; move DOMtrue at bottom; simpl in DOMtrue.
+               specialize (DOMtrue ((b1 - sizeM2)%positive)).
+               rewrite H in DOMtrue. rewrite orb_true_r in DOMtrue.
+               apply handy_lemma; subst sizeM2; try apply DOMtrue; auto.
+         }
+         apply SMvalNu'. generalize H; unfold RNG, DomTgt.
+         subst nu23'. unfold change_ext; destruct nu23.
+         simpl. rewrite HeqextT23.
+         intros H0.
+         apply orb_true_iff in H0; destruct H0. 
+         destruct ExtIncr as [extincr [intincr [? [? [locS [locT [? [? [? ? ]]]]]]]]]; simpl in *.
+         rewrite <- locT. rewrite H0; auto.
+         rewrite H0; apply orb_true_r.
+       }
+       split.
+       split.
+       (* SM_wd 12*)
+       { exact SMWD12'. }
+       split.
+       (* SM_wd 23*)
+       { exact SMWD23'. }
+       split.
+       (* locBlocksTgt = locBlocksSrc *)
+       { subst nu12' nu23'. unfold change_ext; destruct nu12, nu23; simpl.  
+         apply GlueInv.
+       }
+       (* locBlocksTgt = locBlocksSrc *)
+       split.
+       {
+         destruct GlueInv as [? [extEq [? ?]]].
+         subst nu23' nu12'; unfold change_ext; destruct nu23, nu12; subst extS23 extT12; simpl.
+         simpl in extEq; rewrite extEq; auto.
+       }
+       split.
+       (* pubBlocksTgt -> pubBlocksSrc *)
+       { subst nu12' nu23'. unfold change_ext; destruct nu12, nu23; simpl.  
+         apply GlueInv.
+       }
+       (* frgnBlocksTgt -> frgnBlocksSrc *)
+       { subst nu12' nu23'. unfold change_ext; destruct nu12, nu23; simpl.  
+         apply GlueInv.
+       }
+       split.
+       (* Norm *)
+       { subst nu12' nu23'. unfold change_ext; destruct nu12, nu23; simpl. 
+         eapply MKI_norm; subst j k; eauto. 
+
+         (* Proveing 
+          * forall (b : block) (p : block * Z),
+          * extern_of0 b = Some p -> (b < Mem.nextblock m2)%positive *)
+         intros b p H.  destruct p.
+         eapply SMV23. eapply as_inj_DomRng.
+         unfold as_inj, join; simpl. simpl in *; erewrite H; eauto.
+         assumption.
+       }
+       split.
+       { exact UnchPrivSrc12. }
+       (* Mem.unchanged_on *) (*NOTE: hey both Mem.unchanged_on look very alike! *)
+       split.
+       { exact UnchLOOR12.
+       }
+       split.
+       { intros; subst nu12';
+         eapply destruct_sminj12; eauto.
+       }
+       { clear SMWD12 SMWD12' SMWD23'.
+         intros; subst nu23' j k l';
+         edestruct destruct_sminj23; eauto.
+         right; destruct H0 as [b1 rest]; exists b1, d2; exact rest.
+       }
+Qed.
+
+Lemma EFF_interp_II: forall m1 m2 nu12 
+                             (MInj12 : Mem.inject (as_inj nu12) m1 m2) m1'
+                             (Fwd1: mem_forward m1 m1') nu23 m3
+                             (MInj23 : Mem.inject (as_inj nu23) m2 m3) m3'
+                             (Fwd3: mem_forward m3 m3')
+                              nu' (WDnu' : SM_wd nu')
+                             (SMvalNu' : sm_valid nu' m1' m3')
+                             (MemInjNu' : Mem.inject (as_inj nu') m1' m3')
+                             
+                             (ExtIncr: extern_incr (compose_sm nu12 nu23) nu')
+                             (Pure: pure_comp_ext nu12 nu23 m1 m2)
+                             (SMV12: sm_valid nu12 m1 m2)
+                             (SMV23: sm_valid nu23 m2 m3)
+                             (UnchPrivSrc: Mem.unchanged_on (fun b ofs => locBlocksSrc (compose_sm nu12 nu23) b = true /\ 
+                                                      pubBlocksSrc (compose_sm nu12 nu23) b = false) m1 m1') 
+                             (UnchLOOR13: Mem.unchanged_on (local_out_of_reach (compose_sm nu12 nu23) m1) m3 m3')
+
+                             (GlueInvNu: SM_wd nu12 /\ SM_wd nu23 /\
+                                         locBlocksTgt nu12 = locBlocksSrc nu23 /\
+                                         extBlocksTgt nu12 = extBlocksSrc nu23 /\
+                                         (forall b, pubBlocksTgt nu12 b = true -> 
+                                                    pubBlocksSrc nu23 b = true) /\
+                                         (forall b, frgnBlocksTgt nu12 b = true -> 
+                                                    frgnBlocksSrc nu23 b = true))
+                             (Norm12: forall b1 b2 d1, extern_of nu12 b1 = Some(b2,d1) ->
+                                             exists b3 d2, extern_of nu23 b2 = Some(b3, d2))
+                             (full: full_ext nu12 nu23),
+     exists m2', exists nu12', exists nu23', nu'=compose_sm nu12' nu23' /\
+                             extern_incr nu12 nu12' /\ extern_incr nu23 nu23' /\
+                             Mem.inject (as_inj nu12') m1' m2' /\ mem_forward m2 m2' /\
+                             Mem.inject (as_inj nu23') m2' m3' /\
+                             sm_valid nu12' m1' m2' /\ sm_valid nu23' m2' m3' /\
+                             (SM_wd nu12' /\ SM_wd nu23' /\
+                              locBlocksTgt nu12' = locBlocksSrc nu23' /\
+                              extBlocksTgt nu12' = extBlocksSrc nu23' /\
+                              (forall b, pubBlocksTgt nu12' b = true -> 
+                                         pubBlocksSrc nu23' b = true) /\
+                              (forall b, frgnBlocksTgt nu12' b = true -> 
+                                         frgnBlocksSrc nu23' b = true)) /\
+                             (forall b1 b2 d1, extern_of nu12' b1 = Some(b2,d1) ->
+                                     exists b3 d2, extern_of nu23' b2 = Some(b3, d2)) /\ 
+                              Mem.unchanged_on (fun b ofs => locBlocksSrc nu23 b = true /\ 
+                                                             pubBlocksSrc nu23 b = false) m2 m2' /\
+                              Mem.unchanged_on (local_out_of_reach nu12 m1) m2 m2' 
+                          (* /\ Mem.unchanged_on (local_out_of_reach nu23 m2) m3 m3'*).
+Proof. intros.
+  destruct (EFF_interp_II_strong _ _ _ MInj12 _ Fwd1 _ _ MInj23 _ 
+              Fwd3 _ WDnu' SMvalNu' MemInjNu' ExtIncr
+              Pure SMV12 SMV23 UnchPrivSrc UnchLOOR13 GlueInvNu Norm12 full)
+  as [m2' [nu12' [nu23' [A [B [C [D [E [F [G [H [I [J [K [L [M ]]]]]]]]]]]]]]]].
+  exists m2', nu12', nu23'. intuition.
+Qed.
+
+
+
